Micro_C_Examples/C_Array_Examples.thy
@@ -1,12 +1,9 @@
-(* Copyright Amazon.com, Inc. or its affiliates. All Rights Reserved.
-   SPDX-License-Identifier: MIT *)
-
 theory C_Array_Examples
   imports
     Simple_C_Functions 
 begin
 
-section \<open>C Array Verification\<close>
+section \<open>C array verification\<close>
 
 text \<open>
   This theory demonstrates verification of C array indexing operations.
@@ -21,16 +18,16 @@ definition list_fill_prefix :: \<open>nat \<Rightarrow> 'a \<Rightarrow> 'a list
 
 lemma list_fill_prefix_length [simp]:
   assumes \<open>k \<le> length xs\<close>
-  shows \<open>length (list_fill_prefix k v xs) = length xs\<close>
-  using assms by (simp add: list_fill_prefix_def)
+    shows \<open>length (list_fill_prefix k v xs) = length xs\<close>
+using assms by (simp add: list_fill_prefix_def)
 
 lemma list_fill_prefix_zero [simp]:
-  \<open>list_fill_prefix 0 v xs = xs\<close>
-  by (simp add: list_fill_prefix_def)
+  shows \<open>list_fill_prefix 0 v xs = xs\<close>
+by (simp add: list_fill_prefix_def)
 
 lemma list_fill_prefix_step:
   assumes \<open>k < length xs\<close>
-  shows \<open>(list_fill_prefix k v xs)[k := v] = list_fill_prefix (Suc k) v xs\<close>
+    shows \<open>(list_fill_prefix k v xs)[k := v] = list_fill_prefix (Suc k) v xs\<close>
 proof -
   have \<open>drop k xs = xs ! k # drop (Suc k) xs\<close>
     using assms by (simp add: Cons_nth_drop_Suc)
@@ -46,17 +43,18 @@ definition list_copy_prefix :: \<open>nat \<Rightarrow> 'a list \<Rightarrow> 'a
   \<open>list_copy_prefix k src dst \<equiv> take k src @ drop k dst\<close>
 
 lemma list_copy_prefix_length [simp]:
-  assumes \<open>k \<le> length src\<close> \<open>k \<le> length dst\<close>
-  shows \<open>length (list_copy_prefix k src dst) = length dst\<close>
-  using assms by (simp add: list_copy_prefix_def)
+  assumes \<open>k \<le> length src\<close>
+      and \<open>k \<le> length dst\<close>
+    shows \<open>length (list_copy_prefix k src dst) = length dst\<close>
+using assms by (simp add: list_copy_prefix_def)
 
 lemma list_copy_prefix_zero [simp]:
-  \<open>list_copy_prefix 0 src dst = dst\<close>
-  by (simp add: list_copy_prefix_def)
+  shows \<open>list_copy_prefix 0 src dst = dst\<close>
+by (simp add: list_copy_prefix_def)
 
 lemma list_copy_prefix_step:
   assumes \<open>k < length src\<close> \<open>k < length dst\<close>
-  shows \<open>(list_copy_prefix k src dst)[k := src ! k] = list_copy_prefix (Suc k) src dst\<close>
+    shows \<open>(list_copy_prefix k src dst)[k := src ! k] = list_copy_prefix (Suc k) src dst\<close>
 proof -
   have drop_eq: \<open>drop k dst = dst ! k # drop (Suc k) dst\<close>
     using assms by (simp add: Cons_nth_drop_Suc)
@@ -73,17 +71,17 @@ context c_verification_ctx begin
 subsection \<open>C Array Functions\<close>
 
 micro_c_translate \<open>
-int read_at(int *arr, int idx) {
-  return arr[idx];
-}
+  int read_at(int *arr, int idx) {
+    return arr[idx];
+  }
 \<close>
 
 thm c_read_at_def
 
 micro_c_translate \<open>
-void write_at(int *arr, int idx, int val) {
-  arr[idx] = val;
-}
+  void write_at(int *arr, int idx, int val) {
+    arr[idx] = val;
+  }
 \<close>
 
 thm c_write_at_def
@@ -96,8 +94,7 @@ text \<open>
   The @{const c_idx_to_nat} function converts the C integer index to a natural number.
 \<close>
 
-definition c_read_at_contract ::
-    \<open>('addr, 'gv, c_int list) Global_Store.ref \<Rightarrow> c_int \<Rightarrow>
+definition c_read_at_contract :: \<open>('addr, 'gv, c_int list) Global_Store.ref \<Rightarrow> c_int \<Rightarrow>
      'gv \<Rightarrow> c_int list \<Rightarrow> ('s, c_int, 'b) function_contract\<close> where
   [crush_contracts]: \<open>c_read_at_contract arr idx g vs \<equiv>
     let pre  = arr \<mapsto>\<langle>\<top>\<rangle> g\<down>vs \<star> \<langle>c_idx_to_nat idx < length vs\<rangle>;
@@ -107,9 +104,7 @@ ucincl_auto c_read_at_contract
 
 lemma c_read_at_spec:
   shows \<open>\<Gamma>; c_read_at arr idx \<Turnstile>\<^sub>F c_read_at_contract arr idx g vs\<close>
-  apply (crush_boot f: c_read_at_def contract: c_read_at_contract_def)
-  apply crush_base
-  done
+by (crush_boot f: c_read_at_def contract: c_read_at_contract_def) crush_base
 
 subsection \<open>Array Fill (memset-style)\<close>
 
@@ -119,23 +114,22 @@ text \<open>
 \<close>
 
 micro_c_translate \<open>
-void array_fill(int *arr, int val, int n) {
-  for (int i = 0; i < n; i++) {
-    arr[i] = val;
+  void array_fill(int *arr, int val, int n) {
+    for (int i = 0; i < n; i++) {
+      arr[i] = val;
+    }
   }
-}
 \<close>
 
 thm c_array_fill_def
 
-definition c_array_fill_contract ::
-    \<open>('addr, 'gv, c_int list) Global_Store.ref \<Rightarrow> c_int \<Rightarrow> c_int \<Rightarrow>
+definition c_array_fill_contract :: \<open>('addr, 'gv, c_int list) Global_Store.ref \<Rightarrow> c_int \<Rightarrow> c_int \<Rightarrow>
      'gv \<Rightarrow> c_int list \<Rightarrow> ('s, 'a, 'b) function_contract\<close> where
   \<open>c_array_fill_contract arr val n g vs \<equiv>
     let pre  = arr \<mapsto>\<langle>\<top>\<rangle> g\<down>vs \<star>
                \<langle>c_idx_to_nat n \<le> length vs\<rangle> \<star>
                can_alloc_reference;
-        post = \<lambda>_. (\<Squnion> g'. arr \<mapsto>\<langle>\<top>\<rangle> g'\<down>(list_fill_prefix (c_idx_to_nat n) val vs)) \<star>
+        post = \<lambda>_. (\<Squnion>g'. arr \<mapsto>\<langle>\<top>\<rangle> g'\<down>(list_fill_prefix (c_idx_to_nat n) val vs)) \<star>
                can_alloc_reference
      in make_function_contract pre post\<close>
 ucincl_auto c_array_fill_contract
@@ -150,10 +144,7 @@ lemma c_array_fill_spec:
         and \<tau>=\<open>\<lambda>_. \<langle>False\<rangle>\<close>
         and \<theta>=\<open>\<lambda>_. \<langle>False\<rangle>\<close>
       in wp_raw_for_loop_framedI'\<close>)
-  using unat_lt2p[of n]
-  apply (auto simp add: list_fill_prefix_step unat_of_nat_eq)
-  apply crush_base
-  apply (simp add: list_fill_prefix_step)
+  using unat_lt2p[of n] apply (crush_base simp add: list_fill_prefix_step unat_of_nat_eq)
   done
 
 subsection \<open>Array Copy (memcpy-style)\<close>
@@ -164,20 +155,18 @@ text \<open>
 \<close>
 
 micro_c_translate \<open>
-void array_copy(int *dst, int *src, int n) {
-  for (int i = 0; i < n; i++) {
-    dst[i] = src[i];
+  void array_copy(int *dst, int *src, int n) {
+    for (int i = 0; i < n; i++) {
+      dst[i] = src[i];
+    }
   }
-}
 \<close>
 
 thm c_array_copy_def
 
-definition c_array_copy_contract ::
-    \<open>('addr, 'gv, c_int list) Global_Store.ref \<Rightarrow>
-     ('addr, 'gv, c_int list) Global_Store.ref \<Rightarrow> c_int \<Rightarrow>
-     'gv \<Rightarrow> c_int list \<Rightarrow> 'gv \<Rightarrow> c_int list \<Rightarrow>
-     ('s, 'a, 'b) function_contract\<close> where
+definition c_array_copy_contract :: \<open>('addr, 'gv, c_int list) Global_Store.ref \<Rightarrow>
+      ('addr, 'gv, c_int list) Global_Store.ref \<Rightarrow> c_int \<Rightarrow> 'gv \<Rightarrow> c_int list \<Rightarrow> 'gv \<Rightarrow>
+      c_int list \<Rightarrow> ('s, 'a, 'b) function_contract\<close> where
   \<open>c_array_copy_contract dst src n gd vd gs vs \<equiv>
     let pre  = dst \<mapsto>\<langle>\<top>\<rangle> gd\<down>vd \<star> src \<mapsto>\<langle>\<top>\<rangle> gs\<down>vs \<star>
                \<langle>c_idx_to_nat n \<le> length vd\<rangle> \<star>
@@ -199,10 +188,7 @@ lemma c_array_copy_spec:
         and \<tau>=\<open>\<lambda>_. \<langle>False\<rangle>\<close>
         and \<theta>=\<open>\<lambda>_. \<langle>False\<rangle>\<close>
       in wp_raw_for_loop_framedI'\<close>)
-  using unat_lt2p[of n]
-  apply (auto simp add: list_copy_prefix_step unat_of_nat_eq)
-  apply crush_base
-  apply (simp add: list_copy_prefix_step)
+  using unat_lt2p[of n] apply (crush_base simp add: list_copy_prefix_step unat_of_nat_eq)
   done
 
 end
