Micro_C_Examples/C_Bitwise_Examples.thy
@@ -1,6 +1,3 @@
-(* Copyright Amazon.com, Inc. or its affiliates. All Rights Reserved.
-   SPDX-License-Identifier: MIT *)
-
 theory C_Bitwise_Examples
   imports
     Simple_C_Functions
@@ -15,15 +12,15 @@ text ‹
   additionally detect negative-operand and overflow UB.
 ›
 
-subsection ‹Unsigned Bitwise Smoke Tests›
+subsection ‹Unsigned bitwise smoke tests›
 
 context c_uint_verification_ctx
 begin
 
 micro_c_translate ‹
-unsigned int u_and(unsigned int a, unsigned int b) {
-  return a & b;
-}
+  unsigned int u_and(unsigned int a, unsigned int b) {
+    return a & b;
+  }
 ›
 
 definition c_u_and_bw_contract ::
@@ -36,18 +33,16 @@ ucincl_auto c_u_and_bw_contract
 
 lemma c_u_and_bw_spec [crush_specs]:
   shows ‹Γ; c_u_and a b ⊨⇩F c_u_and_bw_contract a b›
-  apply (crush_boot f: c_u_and_def contract: c_u_and_bw_contract_def)
-  apply (crush_base simp add: c_unsigned_and_def)
-  done
+by (crush_boot f: c_u_and_def contract: c_u_and_bw_contract_def)
+  (crush_base simp add: c_unsigned_and_def)
 
 micro_c_translate ‹
-unsigned int u_not(unsigned int x) {
-  return ~x;
-}
+  unsigned int u_not(unsigned int x) {
+    return ~x;
+  }
 ›
 
-definition c_u_not_contract ::
-    ‹c_uint ⇒ ('s::{sepalg}, c_uint, 'b) function_contract› where
+definition c_u_not_contract :: ‹c_uint ⇒ ('s::{sepalg}, c_uint, 'b) function_contract› where
   [crush_contracts]: ‹c_u_not_contract x ≡
     let pre  = ⟨True⟩;
         post = λr. ⟨r = NOT x⟩
@@ -56,14 +51,13 @@ ucincl_auto c_u_not_contract
 
 lemma c_u_not_spec [crush_specs]:
   shows ‹Γ; c_u_not x ⊨⇩F c_u_not_contract x›
-  apply (crush_boot f: c_u_not_def contract: c_u_not_contract_def)
-  apply (crush_base simp add: c_unsigned_not_def)
-  done
+by (crush_boot f: c_u_not_def contract: c_u_not_contract_def)
+  (crush_base simp add: c_unsigned_not_def)
 
 micro_c_translate ‹
-unsigned int u_shl(unsigned int x, unsigned int n) {
-  return x << n;
-}
+  unsigned int u_shl(unsigned int x, unsigned int n) {
+    return x << n;
+  }
 ›
 
 definition c_u_shl_contract ::
@@ -76,22 +70,20 @@ ucincl_auto c_u_shl_contract
 
 lemma c_u_shl_spec [crush_specs]:
   shows ‹Γ; c_u_shl x n ⊨⇩F c_u_shl_contract x n›
-  apply (crush_boot f: c_u_shl_def contract: c_u_shl_contract_def)
-  apply (crush_base simp add: c_unsigned_shl_def)
-  done
+by (crush_boot f: c_u_shl_def contract: c_u_shl_contract_def)
+    (crush_base simp add: c_unsigned_shl_def)
 
-subsection ‹Interesting Semantic Examples›
+subsection ‹Interesting semantic examples›
 
 text ‹Mask low byte: result fits in a byte.›
 
 micro_c_translate ‹
-unsigned int mask_low_byte(unsigned int x) {
-  return x & 255;
-}
+  unsigned int mask_low_byte(unsigned int x) {
+    return x & 255;
+  }
 ›
 
-definition c_mask_low_byte_contract ::
-    ‹c_uint ⇒ ('s::{sepalg}, c_uint, 'b) function_contract› where
+definition c_mask_low_byte_contract :: ‹c_uint ⇒ ('s::{sepalg}, c_uint, 'b) function_contract› where
   [crush_contracts]: ‹c_mask_low_byte_contract x ≡
     let pre  = ⟨True⟩;
         post = λr. ⟨unat r < 256⟩
@@ -100,21 +92,18 @@ ucincl_auto c_mask_low_byte_contract
 
 lemma c_mask_low_byte_spec [crush_specs]:
   shows ‹Γ; c_mask_low_byte x ⊨⇩F c_mask_low_byte_contract x›
-  apply (crush_boot f: c_mask_low_byte_def contract: c_mask_low_byte_contract_def)
-  apply (crush_base simp add: c_unsigned_and_def)
-  apply (rule word_unat_and_lt, simp)
-  done
+by (crush_boot f: c_mask_low_byte_def contract: c_mask_low_byte_contract_def)
+    (crush_base simp add: c_unsigned_and_def intro!: word_unat_and_lt)
 
 text ‹Set bit: the bit at position n is set in the result.›
 
 micro_c_translate ‹
-unsigned int set_bit(unsigned int x, unsigned int n) {
-  return x | (1U << n);
-}
+  unsigned int set_bit(unsigned int x, unsigned int n) {
+    return x | (1U << n);
+  }
 ›
 
-definition c_set_bit_contract ::
-    ‹c_uint ⇒ c_uint ⇒ ('s::{sepalg}, c_uint, 'b) function_contract› where
+definition c_set_bit_contract :: ‹c_uint ⇒ c_uint ⇒ ('s::{sepalg}, c_uint, 'b) function_contract› where
   [crush_contracts]: ‹c_set_bit_contract x n ≡
     let pre  = ⟨unat n < 32⟩;
         post = λr. ⟨bit r (unat n)⟩
@@ -124,20 +113,19 @@ ucincl_auto c_set_bit_contract
 lemma c_set_bit_spec [crush_specs]:
   shows ‹Γ; c_set_bit x n ⊨⇩F c_set_bit_contract x n›
   apply (crush_boot f: c_set_bit_def contract: c_set_bit_contract_def)
-  apply (crush_base simp add: c_unsigned_or_def c_unsigned_shl_def)
-  apply (simp add: bit_or_iff bit_push_bit_iff nth_w2p_same)
+  apply (crush_base simp add: c_unsigned_or_def c_unsigned_shl_def bit_or_iff bit_push_bit_iff
+    nth_w2p_same)
   done
 
 text ‹Clear bit: the bit at position n is cleared in the result.›
 
 micro_c_translate ‹
-unsigned int clear_bit(unsigned int x, unsigned int n) {
-  return x & ~(1U << n);
-}
+  unsigned int clear_bit(unsigned int x, unsigned int n) {
+    return x & ~(1U << n);
+  }
 ›
 
-definition c_clear_bit_contract ::
-    ‹c_uint ⇒ c_uint ⇒ ('s::{sepalg}, c_uint, 'b) function_contract› where
+definition c_clear_bit_contract :: ‹c_uint ⇒ c_uint ⇒ ('s::{sepalg}, c_uint, 'b) function_contract› where
   [crush_contracts]: ‹c_clear_bit_contract x n ≡
     let pre  = ⟨unat n < 32⟩;
         post = λr. ⟨¬ bit r (unat n)⟩
@@ -147,13 +135,13 @@ ucincl_auto c_clear_bit_contract
 lemma c_clear_bit_spec [crush_specs]:
   shows ‹Γ; c_clear_bit x n ⊨⇩F c_clear_bit_contract x n›
   apply (crush_boot f: c_clear_bit_def contract: c_clear_bit_contract_def)
-  apply (crush_base simp add: c_unsigned_and_def c_unsigned_not_def c_unsigned_shl_def)
-  apply (simp add: bit_and_iff bit_not_iff bit_push_bit_iff nth_w2p_same)
+  apply (crush_base simp add: c_unsigned_and_def c_unsigned_not_def c_unsigned_shl_def
+      bit_and_iff bit_not_iff bit_push_bit_iff nth_w2p_same)
   done
 
 end
 
-subsection ‹Signed Bitwise›
+subsection ‹Signed bitwise›
 
 context c_verification_ctx
 begin
@@ -161,13 +149,12 @@ begin
 text ‹Signed bitwise AND has no UB precondition.›
 
 micro_c_translate ‹
-int s_and(int a, int b) {
-  return a & b;
-}
+  int s_and(int a, int b) {
+    return a & b;
+  }
 ›
 
-definition c_s_and_contract ::
-    ‹c_int ⇒ c_int ⇒ ('s::{sepalg}, c_int, 'b) function_contract› where
+definition c_s_and_contract :: ‹c_int ⇒ c_int ⇒ ('s::{sepalg}, c_int, 'b) function_contract› where
   [crush_contracts]: ‹c_s_and_contract a b ≡
     let pre  = ⟨True⟩;
         post = λr. ⟨r = a AND b⟩
@@ -176,9 +163,7 @@ ucincl_auto c_s_and_contract
 
 lemma c_s_and_spec [crush_specs]:
   shows ‹Γ; c_s_and a b ⊨⇩F c_s_and_contract a b›
-  apply (crush_boot f: c_s_and_def contract: c_s_and_contract_def)
-  apply (crush_base simp add: c_signed_and_def)
-  done
+by (crush_boot f: c_s_and_def contract: c_s_and_contract_def) (crush_base simp add: c_signed_and_def)
 
 end
 
