Micro_C_Examples/Simple_C_Functions.thy
@@ -1,6 +1,3 @@
-(* Copyright Amazon.com, Inc. or its affiliates. All Rights Reserved.
-   SPDX-License-Identifier: MIT *)
-
 theory Simple_C_Functions
   imports
     "Micro_C_Parsing_Frontend.C_To_Core_Translation"
@@ -8,7 +5,7 @@ theory Simple_C_Functions
     "Micro_Rust_Std_Lib.StdLib_All"
 begin
 
-section \<open>First End-to-End C Verification Example\<close>
+section \<open>First end-to-end C verification example\<close>
 
 text \<open>
   This theory demonstrates end-to-end verification of C source code using
@@ -18,7 +15,7 @@ text \<open>
   \<^enum> Prove the contract using @{text crush_boot} and @{text crush_base}
 \<close>
 
-subsection \<open>Locale Setup\<close>
+subsection \<open>Locale setup\<close>
 
 text \<open>
   The locale provides the reference infrastructure: allocation, dereference,
@@ -29,23 +26,24 @@ text \<open>
 locale c_verification_ctx =
     reference reference_types +
     ref_c_int: reference_allocatable reference_types _ _ _ _ _ _ _ c_int_prism
-  for
-    reference_types :: \<open>'s::{sepalg} \<Rightarrow> 'addr \<Rightarrow> 'gv \<Rightarrow> 'abort \<Rightarrow> 'i prompt \<Rightarrow> 'o prompt_output \<Rightarrow> unit\<close>
-    and c_int_prism :: \<open>('gv, c_int) prism\<close>
+  for reference_types :: \<open>'s::{sepalg} \<Rightarrow> 'addr \<Rightarrow> 'gv \<Rightarrow> 'abort \<Rightarrow> 'i prompt \<Rightarrow>
+      'o prompt_output \<Rightarrow> unit\<close>
+  and c_int_prism :: \<open>('gv, c_int) prism\<close>
 begin
 
 adhoc_overloading store_reference_const \<rightleftharpoons> ref_c_int.new
 adhoc_overloading store_update_const \<rightleftharpoons> update_fun
 
-subsection \<open>C Swap Function\<close>
+subsection \<open>C swap function\<close>
 
 text \<open>Parse the C swap function.\<close>
 micro_c_translate \<open>
-void swap(int *a, int *b) {
-  int t = *a;
-  *a = *b;
-  *b = t;
-}
+
+  void swap(int *a, int *b) {
+    int t = *a;
+    *a = *b;
+    *b = t;
+  }
 \<close>
 
 thm c_swap_def
@@ -55,34 +53,33 @@ text \<open>
   @{text lval} and @{text rval}, after swap the references hold each
   other's original values.
 \<close>
-definition c_swap_contract ::
-    \<open>('addr, 'gv, c_int) Global_Store.ref \<Rightarrow> ('addr, 'gv, c_int) Global_Store.ref \<Rightarrow>
-     'gv \<Rightarrow> 'gv \<Rightarrow> c_int \<Rightarrow> c_int \<Rightarrow> ('s, 'a, 'b) function_contract\<close> where
+definition c_swap_contract :: \<open>('addr, 'gv, c_int) Global_Store.ref \<Rightarrow>
+      ('addr, 'gv, c_int) Global_Store.ref \<Rightarrow> 'gv \<Rightarrow> 'gv \<Rightarrow> c_int \<Rightarrow> c_int \<Rightarrow>
+      ('s, 'a, 'b) function_contract\<close> where
   \<open>c_swap_contract lref rref lg rg lval rval \<equiv>
     let pre  = can_alloc_reference \<star>
-               lref \<mapsto>\<langle>\<top>\<rangle> lg\<down>lval \<star> rref \<mapsto>\<langle>\<top>\<rangle> rg\<down>rval in
-    let post = \<lambda> _.
-               can_alloc_reference \<star>
+               lref \<mapsto>\<langle>\<top>\<rangle> lg\<down>lval \<star> rref \<mapsto>\<langle>\<top>\<rangle> rg\<down>rval;
+        post = \<lambda> _. can_alloc_reference \<star>
                lref \<mapsto>\<langle>\<top>\<rangle> (\<lambda>_. rval) \<sqdot> (lg\<down>lval) \<star>
-               rref \<mapsto>\<langle>\<top>\<rangle> (\<lambda>_. lval) \<sqdot> (rg\<down>rval) in
-    make_function_contract pre post\<close>
+               rref \<mapsto>\<langle>\<top>\<rangle> (\<lambda>_. lval) \<sqdot> (rg\<down>rval)
+     in make_function_contract pre post\<close>
 ucincl_auto c_swap_contract
 
 text \<open>Prove that the C swap function satisfies its contract.\<close>
 lemma c_swap_spec:
   shows \<open>\<Gamma>; c_swap lref rref \<Turnstile>\<^sub>F c_swap_contract lref rref lg rg lval rval\<close>
-  apply (crush_boot f: c_swap_def contract: c_swap_contract_def)
-  apply crush_base
-  done
+by (crush_boot f: c_swap_def contract: c_swap_contract_def) crush_base
 
 subsection \<open>C Max Function\<close>
 
 text \<open>A simple function exercising conditionals and return.\<close>
 micro_c_translate \<open>
-int max(int a, int b) {
-  if (a > b) return a;
-  else return b;
-}
+  int max(int a, int b) {
+    if (a > b)
+      return a;
+    else
+      return b;
+  }
 \<close>
 
 thm c_max_def
@@ -102,17 +99,17 @@ ucincl_auto c_max_contract
 
 lemma c_max_spec [crush_specs]:
   shows \<open>\<Gamma>; c_max a b \<Turnstile>\<^sub>F c_max_contract a b\<close>
-  apply (crush_boot f: c_max_def contract: c_max_contract_def)
-  apply (crush_base simp add: c_signed_less_def)
-  done
+by (crush_boot f: c_max_def contract: c_max_contract_def) (crush_base simp add: c_signed_less_def)
 
-subsection \<open>C Abs Function\<close>
+subsection \<open>C abs function\<close>
 
 micro_c_translate \<open>
-int abs_val(int x) {
-  if (x > 0) return x;
-  else return 0 - x;
-}
+  int abs_val(int x) {
+    if (x > 0)
+      return x;
+    else
+      return 0 - x;
+  }
 \<close>
 
 thm c_abs_val_def
@@ -122,8 +119,7 @@ text \<open>
   overflows when x is the minimum signed value. The precondition
   ensures the negation is safe.
 \<close>
-definition c_abs_val_contract ::
-    \<open>c_int \<Rightarrow> ('s::{sepalg}, c_int, 'b) function_contract\<close> where
+definition c_abs_val_contract :: \<open>c_int \<Rightarrow> ('s::{sepalg}, c_int, 'b) function_contract\<close> where
   [crush_contracts]: \<open>c_abs_val_contract x \<equiv>
     let pre  = \<langle>-(2^31 :: int) < sint x\<rangle>;
         post = \<lambda>r. \<langle>r = (if sint x > sint (0 :: c_int) then x else word_of_int (0 - sint x))\<rangle>
@@ -132,9 +128,8 @@ ucincl_auto c_abs_val_contract
 
 lemma c_abs_val_spec [crush_specs]:
   shows \<open>\<Gamma>; c_abs_val x \<Turnstile>\<^sub>F c_abs_val_contract x\<close>
-  apply (crush_boot f: c_abs_val_def contract: c_abs_val_contract_def)
-  apply (crush_base simp add: c_signed_less_def c_signed_sub_def c_signed_overflow_def Let_def)
-  done
+by (crush_boot f: c_abs_val_def contract: c_abs_val_contract_def) (crush_base simp add:
+  c_signed_less_def c_signed_sub_def c_signed_overflow_def Let_def)
 
 end
 
@@ -149,18 +144,18 @@ text \<open>
 locale c_uint_verification_ctx =
     reference reference_types +
     ref_c_uint: reference_allocatable reference_types _ _ _ _ _ _ _ c_uint_prism
-  for
-    reference_types :: \<open>'s::{sepalg} \<Rightarrow> 'addr \<Rightarrow> 'gv \<Rightarrow> 'abort \<Rightarrow> 'i prompt \<Rightarrow> 'o prompt_output \<Rightarrow> unit\<close>
-    and c_uint_prism :: \<open>('gv, c_uint) prism\<close>
+  for reference_types :: \<open>'s::{sepalg} \<Rightarrow> 'addr \<Rightarrow> 'gv \<Rightarrow> 'abort \<Rightarrow> 'i prompt \<Rightarrow>
+        'o prompt_output \<Rightarrow> unit\<close>
+  and c_uint_prism :: \<open>('gv, c_uint) prism\<close>
 begin
 
 adhoc_overloading store_reference_const \<rightleftharpoons> ref_c_uint.new
 adhoc_overloading store_update_const \<rightleftharpoons> update_fun
 
 micro_c_translate \<open>
-unsigned int u_add(unsigned int a, unsigned int b) {
-  return a + b;
-}
+  unsigned int u_add(unsigned int a, unsigned int b) {
+    return a + b;
+  }
 \<close>
 
 thm c_u_add_def
@@ -170,8 +165,7 @@ text \<open>
   always @{term \<open>a + b\<close>} (Isabelle word addition already wraps).
   No overflow precondition needed.
 \<close>
-definition c_u_add_contract ::
-    \<open>c_uint \<Rightarrow> c_uint \<Rightarrow> ('s::{sepalg}, c_uint, 'b) function_contract\<close> where
+definition c_u_add_contract :: \<open>c_uint \<Rightarrow> c_uint \<Rightarrow> ('s::{sepalg}, c_uint, 'b) function_contract\<close> where
   [crush_contracts]: \<open>c_u_add_contract a b \<equiv>
     let pre  = \<langle>True\<rangle>;
         post = \<lambda>r. \<langle>r = a + b\<rangle>
@@ -180,21 +174,20 @@ ucincl_auto c_u_add_contract
 
 lemma c_u_add_spec [crush_specs]:
   shows \<open>\<Gamma>; c_u_add a b \<Turnstile>\<^sub>F c_u_add_contract a b\<close>
-  apply (crush_boot f: c_u_add_def contract: c_u_add_contract_def)
-  apply (crush_base simp add: c_unsigned_add_def)
-  done
+by (crush_boot f: c_u_add_def contract: c_u_add_contract_def) (crush_base simp add: c_unsigned_add_def)
 
 micro_c_translate \<open>
-unsigned int u_max(unsigned int a, unsigned int b) {
-  if (a > b) return a;
-  else return b;
-}
+  unsigned int u_max(unsigned int a, unsigned int b) {
+    if (a > b)
+      return a;
+    else
+      return b;
+  }
 \<close>
 
 thm c_u_max_def
 
-definition c_u_max_contract ::
-    \<open>c_uint \<Rightarrow> c_uint \<Rightarrow> ('s::{sepalg}, c_uint, 'b) function_contract\<close> where
+definition c_u_max_contract :: \<open>c_uint \<Rightarrow> c_uint \<Rightarrow> ('s::{sepalg}, c_uint, 'b) function_contract\<close> where
   [crush_contracts]: \<open>c_u_max_contract a b \<equiv>
     let pre  = \<langle>True\<rangle>;
         post = \<lambda>r. \<langle>r = (if b < a then a else b)\<rangle>
@@ -203,92 +196,86 @@ ucincl_auto c_u_max_contract
 
 lemma c_u_max_spec [crush_specs]:
   shows \<open>\<Gamma>; c_u_max a b \<Turnstile>\<^sub>F c_u_max_contract a b\<close>
-  apply (crush_boot f: c_u_max_def contract: c_u_max_contract_def)
-  apply (crush_base simp add: c_unsigned_less_def)
-  done
+by (crush_boot f: c_u_max_def contract: c_u_max_contract_def) (crush_base simp add: c_unsigned_less_def)
 
-subsection \<open>Comma Operator\<close>
+subsection \<open>Comma operator\<close>
 
 micro_c_translate \<open>
-unsigned int comma_test(unsigned int a, unsigned int b) {
+
+  unsigned int comma_test(unsigned int a, unsigned int b) {
     unsigned int x = (a, b);
     return x;
-}
+  }
 \<close>
 
-definition c_comma_test_contract ::
-    \<open>c_uint \<Rightarrow> c_uint \<Rightarrow> ('s::{sepalg}, c_uint, 'b) function_contract\<close> where
+definition c_comma_test_contract :: \<open>c_uint \<Rightarrow> c_uint \<Rightarrow> ('s::{sepalg}, c_uint, 'b) function_contract\<close> where
   [crush_contracts]: \<open>c_comma_test_contract a b \<equiv>
     let pre  = can_alloc_reference;
-        post = \<lambda>r. can_alloc_reference \<star> \<langle>r = b\<rangle>
+        post = \<lambda>r. can_alloc_reference \<star>
+               \<langle>r = b\<rangle>
      in make_function_contract pre post\<close>
 ucincl_auto c_comma_test_contract
 
 lemma c_comma_test_spec [crush_specs]:
   shows \<open>\<Gamma>; c_comma_test a b \<Turnstile>\<^sub>F c_comma_test_contract a b\<close>
-  apply (crush_boot f: c_comma_test_def contract: c_comma_test_contract_def)
-  apply crush_base
-  done
+by (crush_boot f: c_comma_test_def contract: c_comma_test_contract_def) crush_base
 
 subsection \<open>Multiple Declarations\<close>
 
 micro_c_translate \<open>
-unsigned int multi_decl_add(unsigned int a, unsigned int b) {
+  unsigned int multi_decl_add(unsigned int a, unsigned int b) {
     unsigned int x = a, y = b;
     return x + y;
-}
+  }
 \<close>
 
-definition c_multi_decl_add_contract ::
-    \<open>c_uint \<Rightarrow> c_uint \<Rightarrow> ('s::{sepalg}, c_uint, 'b) function_contract\<close> where
+definition c_multi_decl_add_contract :: \<open>c_uint \<Rightarrow> c_uint \<Rightarrow> ('s::{sepalg}, c_uint, 'b) function_contract\<close> where
   [crush_contracts]: \<open>c_multi_decl_add_contract a b \<equiv>
     let pre  = can_alloc_reference;
-        post = \<lambda>r. can_alloc_reference \<star> \<langle>r = a + b\<rangle>
+        post = \<lambda>r. can_alloc_reference \<star>
+               \<langle>r = a + b\<rangle>
      in make_function_contract pre post\<close>
 ucincl_auto c_multi_decl_add_contract
 
 lemma c_multi_decl_add_spec [crush_specs]:
   shows \<open>\<Gamma>; c_multi_decl_add a b \<Turnstile>\<^sub>F c_multi_decl_add_contract a b\<close>
-  apply (crush_boot f: c_multi_decl_add_def contract: c_multi_decl_add_contract_def)
-  apply (crush_base simp add: c_unsigned_add_def)
-  done
-
-subsection \<open>Pre-Increment\<close>
+by (crush_boot f: c_multi_decl_add_def contract: c_multi_decl_add_contract_def)
+  (crush_base simp add: c_unsigned_add_def)
+  
+subsection \<open>Pre-increment\<close>
 
 micro_c_translate \<open>
-unsigned int pre_inc_test(unsigned int init) {
+  unsigned int pre_inc_test(unsigned int init) {
     unsigned int x = init;
     unsigned int r = ++x;
     return r;
-}
+  }
 \<close>
 
-definition c_pre_inc_test_contract ::
-    \<open>c_uint \<Rightarrow> ('s::{sepalg}, c_uint, 'b) function_contract\<close> where
+definition c_pre_inc_test_contract :: \<open>c_uint \<Rightarrow> ('s::{sepalg}, c_uint, 'b) function_contract\<close> where
   [crush_contracts]: \<open>c_pre_inc_test_contract init \<equiv>
     let pre  = can_alloc_reference;
-        post = \<lambda>r. can_alloc_reference \<star> \<langle>r = init + 1\<rangle>
+        post = \<lambda>r. can_alloc_reference \<star>
+               \<langle>r = init + 1\<rangle>
      in make_function_contract pre post\<close>
 ucincl_auto c_pre_inc_test_contract
 
 lemma c_pre_inc_test_spec [crush_specs]:
   shows \<open>\<Gamma>; c_pre_inc_test init \<Turnstile>\<^sub>F c_pre_inc_test_contract init\<close>
-  apply (crush_boot f: c_pre_inc_test_def contract: c_pre_inc_test_contract_def)
-  apply (crush_base simp add: c_unsigned_add_def)
-  done
-
+by (crush_boot f: c_pre_inc_test_def contract: c_pre_inc_test_contract_def)
+  (crush_base simp add: c_unsigned_add_def)
+  
 subsection \<open>Post-Increment\<close>
 
 micro_c_translate \<open>
-unsigned int post_inc_test(unsigned int init) {
+  unsigned int post_inc_test(unsigned int init) {
     unsigned int x = init;
     unsigned int r = x++;
     return r;
-}
+  }
 \<close>
 
-definition c_post_inc_test_contract ::
-    \<open>c_uint \<Rightarrow> ('s::{sepalg}, c_uint, 'b) function_contract\<close> where
+definition c_post_inc_test_contract :: \<open>c_uint \<Rightarrow> ('s::{sepalg}, c_uint, 'b) function_contract\<close> where
   [crush_contracts]: \<open>c_post_inc_test_contract init \<equiv>
     let pre  = can_alloc_reference;
         post = \<lambda>r. can_alloc_reference \<star> \<langle>r = init\<rangle>
@@ -297,22 +284,20 @@ ucincl_auto c_post_inc_test_contract
 
 lemma c_post_inc_test_spec [crush_specs]:
   shows \<open>\<Gamma>; c_post_inc_test init \<Turnstile>\<^sub>F c_post_inc_test_contract init\<close>
-  apply (crush_boot f: c_post_inc_test_def contract: c_post_inc_test_contract_def)
-  apply (crush_base simp add: c_unsigned_add_def)
-  done
+by (crush_boot f: c_post_inc_test_def contract: c_post_inc_test_contract_def)
+  (crush_base simp add: c_unsigned_add_def)
 
 subsection \<open>Post-Decrement\<close>
 
 micro_c_translate \<open>
-unsigned int post_dec_test(unsigned int init) {
+  unsigned int post_dec_test(unsigned int init) {
     unsigned int x = init;
     unsigned int r = x--;
     return r;
-}
+  }
 \<close>
 
-definition c_post_dec_test_contract ::
-    \<open>c_uint \<Rightarrow> ('s::{sepalg}, c_uint, 'b) function_contract\<close> where
+definition c_post_dec_test_contract :: \<open>c_uint \<Rightarrow> ('s::{sepalg}, c_uint, 'b) function_contract\<close> where
   [crush_contracts]: \<open>c_post_dec_test_contract init \<equiv>
     let pre  = can_alloc_reference;
         post = \<lambda>r. can_alloc_reference \<star> \<langle>r = init\<rangle>
@@ -321,21 +306,21 @@ ucincl_auto c_post_dec_test_contract
 
 lemma c_post_dec_test_spec [crush_specs]:
   shows \<open>\<Gamma>; c_post_dec_test init \<Turnstile>\<^sub>F c_post_dec_test_contract init\<close>
-  apply (crush_boot f: c_post_dec_test_def contract: c_post_dec_test_contract_def)
-  apply (crush_base simp add: c_unsigned_sub_def)
-  done
+by (crush_boot f: c_post_dec_test_def contract: c_post_dec_test_contract_def)
+  (crush_base simp add: c_unsigned_sub_def)
 
 subsection \<open>Not-Equal Operator\<close>
 
 micro_c_translate \<open>
-unsigned int neq_test(unsigned int a, unsigned int b) {
-  if (a != b) return 1;
-  else return 0;
-}
+  unsigned int neq_test(unsigned int a, unsigned int b) {
+    if (a != b)
+      return 1;
+    else
+      return 0;
+  }
 \<close>
 
-definition c_neq_test_contract ::
-    \<open>c_uint \<Rightarrow> c_uint \<Rightarrow> ('s::{sepalg}, c_uint, 'b) function_contract\<close> where
+definition c_neq_test_contract :: \<open>c_uint \<Rightarrow> c_uint \<Rightarrow> ('s::{sepalg}, c_uint, 'b) function_contract\<close> where
   [crush_contracts]: \<open>c_neq_test_contract a b \<equiv>
     let pre  = \<langle>True\<rangle>;
         post = \<lambda>r. \<langle>r = (if a \<noteq> b then 1 else 0)\<rangle>
@@ -344,21 +329,21 @@ ucincl_auto c_neq_test_contract
 
 lemma c_neq_test_spec [crush_specs]:
   shows \<open>\<Gamma>; c_neq_test a b \<Turnstile>\<^sub>F c_neq_test_contract a b\<close>
-  apply (crush_boot f: c_neq_test_def contract: c_neq_test_contract_def)
-  apply (crush_base simp add: c_unsigned_neq_def)
-  done
+by (crush_boot f: c_neq_test_def contract: c_neq_test_contract_def)
+  (crush_base simp add: c_unsigned_neq_def)
 
 subsection \<open>Logical NOT\<close>
 
 micro_c_translate \<open>
-unsigned int is_zero(unsigned int x) {
-  if (!x) return 1;
-  else return 0;
-}
+  unsigned int is_zero(unsigned int x) {
+    if (!x)
+      return 1;
+    else
+      return 0;
+  }
 \<close>
 
-definition c_is_zero_contract ::
-    \<open>c_uint \<Rightarrow> ('s::{sepalg}, c_uint, 'b) function_contract\<close> where
+definition c_is_zero_contract :: \<open>c_uint \<Rightarrow> ('s::{sepalg}, c_uint, 'b) function_contract\<close> where
   [crush_contracts]: \<open>c_is_zero_contract x \<equiv>
     let pre  = \<langle>True\<rangle>;
         post = \<lambda>r. \<langle>r = (if x = 0 then 1 else 0)\<rangle>
@@ -367,14 +352,15 @@ ucincl_auto c_is_zero_contract
 
 lemma c_is_zero_spec [crush_specs]:
   shows \<open>\<Gamma>; c_is_zero x \<Turnstile>\<^sub>F c_is_zero_contract x\<close>
-  apply (crush_boot f: c_is_zero_def contract: c_is_zero_contract_def)
-  apply (crush_base simp add: c_unsigned_eq_def)
-  done
+by (crush_boot f: c_is_zero_def contract: c_is_zero_contract_def)
+  (crush_base simp add: c_unsigned_eq_def)
 
-subsection \<open>Unary Plus\<close>
+subsection \<open>Unary plus\<close>
 
 micro_c_translate \<open>
-unsigned int uplus(unsigned int x) { return +x; }
+  unsigned int uplus(unsigned int x) {
+    return +x;
+  }
 \<close>
 
 definition c_uplus_contract ::
@@ -387,16 +373,14 @@ ucincl_auto c_uplus_contract
 
 lemma c_uplus_spec [crush_specs]:
   shows \<open>\<Gamma>; c_uplus x \<Turnstile>\<^sub>F c_uplus_contract x\<close>
-  apply (crush_boot f: c_uplus_def contract: c_uplus_contract_def)
-  apply crush_base
-  done
+by (crush_boot f: c_uplus_def contract: c_uplus_contract_def) crush_base
 
-subsection \<open>Ternary Operator\<close>
+subsection \<open>Ternary operator\<close>
 
 micro_c_translate \<open>
-unsigned int ternary_max(unsigned int a, unsigned int b) {
-  return (a > b) ? a : b;
-}
+  unsigned int ternary_max(unsigned int a, unsigned int b) {
+    return (a > b) ? a : b;
+  }
 \<close>
 
 definition c_ternary_max_contract ::
@@ -409,44 +393,44 @@ ucincl_auto c_ternary_max_contract
 
 lemma c_ternary_max_spec [crush_specs]:
   shows \<open>\<Gamma>; c_ternary_max a b \<Turnstile>\<^sub>F c_ternary_max_contract a b\<close>
-  apply (crush_boot f: c_ternary_max_def contract: c_ternary_max_contract_def)
-  apply (crush_base simp add: c_unsigned_less_def)
-  done
+by (crush_boot f: c_ternary_max_def contract: c_ternary_max_contract_def)
+    (crush_base simp add: c_unsigned_less_def)
 
-subsection \<open>Compound Assignment\<close>
+subsection \<open>Compound assignment\<close>
 
 micro_c_translate \<open>
-unsigned int add_assign(unsigned int a, unsigned int b) {
-  unsigned int x = a;
-  x += b;
-  return x;
-}
+  unsigned int add_assign(unsigned int a, unsigned int b) {
+    unsigned int x = a;
+    x += b;
+    return x;
+  }
 \<close>
 
-definition c_add_assign_contract ::
-    \<open>c_uint \<Rightarrow> c_uint \<Rightarrow> ('s::{sepalg}, c_uint, 'b) function_contract\<close> where
+definition c_add_assign_contract :: \<open>c_uint \<Rightarrow> c_uint \<Rightarrow>
+      ('s::{sepalg}, c_uint, 'b) function_contract\<close> where
   [crush_contracts]: \<open>c_add_assign_contract a b \<equiv>
     let pre  = can_alloc_reference;
-        post = \<lambda>r. can_alloc_reference \<star> \<langle>r = a + b\<rangle>
+        post = \<lambda>r. can_alloc_reference \<star>
+               \<langle>r = a + b\<rangle>
      in make_function_contract pre post\<close>
 ucincl_auto c_add_assign_contract
 
 lemma c_add_assign_spec [crush_specs]:
   shows \<open>\<Gamma>; c_add_assign a b \<Turnstile>\<^sub>F c_add_assign_contract a b\<close>
-  apply (crush_boot f: c_add_assign_def contract: c_add_assign_contract_def)
-  apply (crush_base simp add: c_unsigned_add_def)
-  done
+by (crush_boot f: c_add_assign_def contract: c_add_assign_contract_def)
+  (crush_base simp add: c_unsigned_add_def)
 
-subsection \<open>Cast: Widen Unsigned Char to Unsigned Int\<close>
+subsection \<open>Cast: widen unsigned char to unsigned int\<close>
 
 micro_c_translate \<open>
-unsigned int widen_char(unsigned char x) { return (unsigned int)x; }
+  unsigned int widen_char(unsigned char x) {
+    return (unsigned int)x;
+  }
 \<close>
 
 thm c_widen_char_def
 
-definition c_widen_char_contract ::
-    \<open>c_char \<Rightarrow> ('s::{sepalg}, c_uint, 'b) function_contract\<close> where
+definition c_widen_char_contract :: \<open>c_char \<Rightarrow> ('s::{sepalg}, c_uint, 'b) function_contract\<close> where
   [crush_contracts]: \<open>c_widen_char_contract x \<equiv>
     let pre  = \<langle>True\<rangle>;
         post = \<lambda>r. \<langle>r = ucast x\<rangle>
@@ -455,20 +439,19 @@ ucincl_auto c_widen_char_contract
 
 lemma c_widen_char_spec [crush_specs]:
   shows \<open>\<Gamma>; c_widen_char x \<Turnstile>\<^sub>F c_widen_char_contract x\<close>
-  apply (crush_boot f: c_widen_char_def contract: c_widen_char_contract_def)
-  apply (crush_base simp add: c_ucast_def)
-  done
+by (crush_boot f: c_widen_char_def contract: c_widen_char_contract_def) (crush_base simp add: c_ucast_def)
 
-subsection \<open>Integer Literal Suffix\<close>
+subsection \<open>Integer literal suffix\<close>
 
 micro_c_translate \<open>
-unsigned int suffix_add(unsigned int x) { return x + 1U; }
+  unsigned int suffix_add(unsigned int x) {
+    return x + 1U;
+  }
 \<close>
 
 thm c_suffix_add_def
 
-definition c_suffix_add_contract ::
-    \<open>c_uint \<Rightarrow> ('s::{sepalg}, c_uint, 'b) function_contract\<close> where
+definition c_suffix_add_contract :: \<open>c_uint \<Rightarrow> ('s::{sepalg}, c_uint, 'b) function_contract\<close> where
   [crush_contracts]: \<open>c_suffix_add_contract x \<equiv>
     let pre  = \<langle>True\<rangle>;
         post = \<lambda>r. \<langle>r = x + 1\<rangle>
@@ -477,42 +460,45 @@ ucincl_auto c_suffix_add_contract
 
 lemma c_suffix_add_spec [crush_specs]:
   shows \<open>\<Gamma>; c_suffix_add x \<Turnstile>\<^sub>F c_suffix_add_contract x\<close>
-  apply (crush_boot f: c_suffix_add_def contract: c_suffix_add_contract_def)
-  apply (crush_base simp add: c_unsigned_add_def)
-  done
+by (crush_boot f: c_suffix_add_def contract: c_suffix_add_contract_def)
+  (crush_base simp add: c_unsigned_add_def)
 
-subsection \<open>Assignment to Parameter\<close>
+subsection \<open>Assignment to parameter\<close>
 
 micro_c_translate \<open>
-unsigned int double_val(unsigned int x) { x = x + x; return x; }
+  unsigned int double_val(unsigned int x) {
+    x = x + x;
+    return x;
+  }
 \<close>
 
 thm c_double_val_def
 
-definition c_double_val_contract ::
-    \<open>c_uint \<Rightarrow> ('s::{sepalg}, c_uint, 'b) function_contract\<close> where
+definition c_double_val_contract :: \<open>c_uint \<Rightarrow> ('s::{sepalg}, c_uint, 'b) function_contract\<close> where
   [crush_contracts]: \<open>c_double_val_contract x \<equiv>
     let pre  = can_alloc_reference;
-        post = \<lambda>r. can_alloc_reference \<star> \<langle>r = x + x\<rangle>
+        post = \<lambda>r. can_alloc_reference \<star>
+               \<langle>r = x + x\<rangle>
      in make_function_contract pre post\<close>
 ucincl_auto c_double_val_contract
 
 lemma c_double_val_spec [crush_specs]:
   shows \<open>\<Gamma>; c_double_val x \<Turnstile>\<^sub>F c_double_val_contract x\<close>
-  apply (crush_boot f: c_double_val_def contract: c_double_val_contract_def)
-  apply (crush_base simp add: c_unsigned_add_def)
-  done
+by (crush_boot f: c_double_val_def contract: c_double_val_contract_def)
+  (crush_base simp add: c_unsigned_add_def)
 
-subsection \<open>Compound Pointer Dereference\<close>
+subsection \<open>Compound pointer dereference\<close>
 
 micro_c_translate \<open>
-unsigned int inc_ptr(unsigned int *p) { *p += 1; return *p; }
+  unsigned int inc_ptr(unsigned int *p) {
+    *p += 1;
+    return *p;
+  }
 \<close>
 
 thm c_inc_ptr_def
 
-definition c_inc_ptr_contract ::
-    \<open>('addr, 'gv, c_uint) Global_Store.ref \<Rightarrow>
+definition c_inc_ptr_contract :: \<open>('addr, 'gv, c_uint) Global_Store.ref \<Rightarrow>
      'gv \<Rightarrow> c_uint \<Rightarrow> ('s::{sepalg}, c_uint, 'b) function_contract\<close> where
   [crush_contracts]: \<open>c_inc_ptr_contract p pg val \<equiv>
     let pre  = p \<mapsto>\<langle>\<top>\<rangle> pg\<down>val;
@@ -522,36 +508,43 @@ ucincl_auto c_inc_ptr_contract
 
 lemma c_inc_ptr_spec [crush_specs]:
   shows \<open>\<Gamma>; c_inc_ptr p \<Turnstile>\<^sub>F c_inc_ptr_contract p pg val\<close>
-  apply (crush_boot f: c_inc_ptr_def contract: c_inc_ptr_contract_def)
-  apply (crush_base simp add: c_unsigned_add_def)
-  done
+by (crush_boot f: c_inc_ptr_def contract: c_inc_ptr_contract_def)
+  (crush_base simp add: c_unsigned_add_def)
 
 subsection \<open>Sizeof\<close>
 
 micro_c_translate \<open>
-unsigned int size_of_int(void) { return sizeof(int); }
+  unsigned int size_of_int(void) {
+    return sizeof(int);
+  }
 \<close>
 
 thm c_size_of_int_def
 
-subsection \<open>Switch Statement\<close>
+subsection \<open>Switch statement\<close>
 
 micro_c_translate \<open>
-unsigned int classify(unsigned int x) {
-  unsigned int result;
-  switch (x) {
-    case 0: result = 10; break;
-    case 1: result = 20; break;
-    default: result = 30; break;
-  }
-  return result;
+  unsigned int classify(unsigned int x) {
+    unsigned int result;
+
+    switch (x) {
+    case 0:
+      result = 10;
+      break;
+    case 1:
+      result = 20;
+      break;
+    default:
+      result = 30;
+      break;
+    }
+    return result;
 }
 \<close>
 
 thm c_classify_def
 
-definition c_classify_contract ::
-    \<open>c_uint \<Rightarrow> ('s::{sepalg}, c_uint, 'b) function_contract\<close> where
+definition c_classify_contract :: \<open>c_uint \<Rightarrow> ('s::{sepalg}, c_uint, 'b) function_contract\<close> where
   [crush_contracts]: \<open>c_classify_contract x \<equiv>
     let pre  = can_alloc_reference;
         post = \<lambda>r. can_alloc_reference \<star> \<langle>r = (if x = 0 then 10 else if x = 1 then 20 else 30)\<rangle>
@@ -560,11 +553,9 @@ ucincl_auto c_classify_contract
 
 lemma c_classify_spec [crush_specs]:
   shows \<open>\<Gamma>; c_classify x \<Turnstile>\<^sub>F c_classify_contract x\<close>
-  apply (crush_boot f: c_classify_def contract: c_classify_contract_def)
-  apply (crush_base)
-  done
+by (crush_boot f: c_classify_def contract: c_classify_contract_def) crush_base
 
-subsection \<open>Address-Of\<close>
+subsection \<open>Address-of\<close>
 
 text \<open>
   Test address-of: @{text "&x"} on a local variable returns the ref itself.
@@ -572,31 +563,30 @@ text \<open>
 \<close>
 
 micro_c_translate \<open>
-unsigned int inc_via_addr(void) {
-  unsigned int x = 5;
-  unsigned int *p = &x;
-  *p = *p + 1;
-  return x;
-}
+  unsigned int inc_via_addr(void) {
+    unsigned int x = 5;
+    unsigned int *p = &x;
+    *p = *p + 1;
+    return x;
+  }
 \<close>
 
 thm c_inc_via_addr_def
 
-definition c_inc_via_addr_contract ::
-    \<open>('s::{sepalg}, c_uint, 'b) function_contract\<close> where
+definition c_inc_via_addr_contract :: \<open>('s::{sepalg}, c_uint, 'b) function_contract\<close> where
   [crush_contracts]: \<open>c_inc_via_addr_contract \<equiv>
     let pre  = can_alloc_reference;
-        post = \<lambda>r. can_alloc_reference \<star> \<langle>r = 6\<rangle>
+        post = \<lambda>r. can_alloc_reference \<star>
+               \<langle>r = 6\<rangle>
      in make_function_contract pre post\<close>
 ucincl_auto c_inc_via_addr_contract
 
 lemma c_inc_via_addr_spec [crush_specs]:
   shows \<open>\<Gamma>; c_inc_via_addr \<Turnstile>\<^sub>F c_inc_via_addr_contract\<close>
-  apply (crush_boot f: c_inc_via_addr_def contract: c_inc_via_addr_contract_def)
-  apply (crush_base simp add: c_unsigned_add_def)
-  done
+by (crush_boot f: c_inc_via_addr_def contract: c_inc_via_addr_contract_def)
+  (crush_base simp add: c_unsigned_add_def)
 
-subsection \<open>Pointer Arithmetic\<close>
+subsection \<open>Pointer arithmetic\<close>
 
 text \<open>
   Test pointer arithmetic: @{text "*(arr + idx)"} reads the element at offset @{text idx}
@@ -604,17 +594,15 @@ text \<open>
 \<close>
 
 micro_c_translate \<open>
-unsigned int ptr_add_read(unsigned int *arr, unsigned int idx) {
-  return *(arr + idx);
-}
+  unsigned int ptr_add_read(unsigned int *arr, unsigned int idx) {
+    return *(arr + idx);
+  }
 \<close>
 
 thm c_ptr_add_read_def
 
-definition c_ptr_add_read_contract ::
-    \<open>('addr, 'gv, c_uint list) Global_Store.ref \<Rightarrow>
-     'gv \<Rightarrow> c_uint list \<Rightarrow> c_uint \<Rightarrow>
-     ('s::{sepalg}, c_uint, 'b) function_contract\<close> where
+definition c_ptr_add_read_contract :: \<open>('addr, 'gv, c_uint list) Global_Store.ref \<Rightarrow> 'gv \<Rightarrow>
+      c_uint list \<Rightarrow> c_uint \<Rightarrow> ('s::{sepalg}, c_uint, 'b) function_contract\<close> where
   [crush_contracts]: \<open>c_ptr_add_read_contract arr ag vs idx \<equiv>
     let pre  = arr \<mapsto>\<langle>\<top>\<rangle> ag\<down>vs \<star> \<langle>c_idx_to_nat idx < length vs\<rangle>;
         post = \<lambda>r. arr \<mapsto>\<langle>\<top>\<rangle> ag\<down>vs \<star> \<langle>r = vs ! c_idx_to_nat idx\<rangle>
@@ -623,11 +611,9 @@ ucincl_auto c_ptr_add_read_contract
 
 lemma c_ptr_add_read_spec [crush_specs]:
   shows \<open>\<Gamma>; c_ptr_add_read arr idx \<Turnstile>\<^sub>F c_ptr_add_read_contract arr ag vs idx\<close>
-  apply (crush_boot f: c_ptr_add_read_def contract: c_ptr_add_read_contract_def)
-  apply crush_base
-  done
+by (crush_boot f: c_ptr_add_read_def contract: c_ptr_add_read_contract_def) crush_base
 
-subsection \<open>Forward-Only Goto\<close>
+subsection \<open>Forward-only goto\<close>
 
 text \<open>
   Test forward-only goto: @{text "goto done"} skips @{text "result = a + b"}
@@ -635,49 +621,52 @@ text \<open>
 \<close>
 
 micro_c_translate \<open>
-unsigned int skip_add(unsigned int a, unsigned int b) {
-  unsigned int result = a;
-  if (b == 0) goto done;
-  result = a + b;
-done:
-  return result;
-}
+  unsigned int skip_add(unsigned int a, unsigned int b) {
+    unsigned int result = a;
+    if (b == 0)
+      goto done;
+    result = a + b;
+  done:
+    return result;
+  }
 \<close>
 
 thm c_skip_add_def
 
-definition c_skip_add_contract ::
-    \<open>c_uint \<Rightarrow> c_uint \<Rightarrow> ('s::{sepalg}, c_uint, 'b) function_contract\<close> where
+definition c_skip_add_contract :: \<open>c_uint \<Rightarrow> c_uint \<Rightarrow> ('s::{sepalg}, c_uint, 'b) function_contract\<close> where
   [crush_contracts]: \<open>c_skip_add_contract a b \<equiv>
     let pre  = can_alloc_reference;
-        post = \<lambda>r. can_alloc_reference \<star> \<langle>r = (if b = 0 then a else a + b)\<rangle>
+        post = \<lambda>r. can_alloc_reference \<star>
+               \<langle>r = (if b = 0 then a else a + b)\<rangle>
      in make_function_contract pre post\<close>
 ucincl_auto c_skip_add_contract
 
 lemma c_skip_add_spec [crush_specs]:
   shows \<open>\<Gamma>; c_skip_add a b \<Turnstile>\<^sub>F c_skip_add_contract a b\<close>
-  apply (crush_boot f: c_skip_add_def contract: c_skip_add_contract_def)
-  apply (crush_base simp add: c_unsigned_eq_def c_unsigned_add_def)
-  done
+by (crush_boot f: c_skip_add_def contract: c_skip_add_contract_def)
+    (crush_base simp add: c_unsigned_eq_def c_unsigned_add_def)
 
 end
 
-section \<open>Fixed-Width Integer Type Verification (uint16_t)\<close>
+section \<open>Fixed-width integer type verification (\<^verbatim>\<open>uint16_t\<close>)\<close>
 
 locale c_ushort_verification_ctx =
     reference reference_types +
     ref_c_ushort: reference_allocatable reference_types _ _ _ _ _ _ _ c_ushort_prism
-  for
-    reference_types :: \<open>'s::{sepalg} \<Rightarrow> 'addr \<Rightarrow> 'gv \<Rightarrow> 'abort \<Rightarrow> 'i prompt \<Rightarrow> 'o prompt_output \<Rightarrow> unit\<close>
-    and c_ushort_prism :: \<open>('gv, c_ushort) prism\<close>
+  for reference_types :: \<open>'s::{sepalg} \<Rightarrow> 'addr \<Rightarrow> 'gv \<Rightarrow> 'abort \<Rightarrow> 'i prompt \<Rightarrow>
+        'o prompt_output \<Rightarrow> unit\<close>
+  and c_ushort_prism :: \<open>('gv, c_ushort) prism\<close>
 begin
 
 adhoc_overloading store_reference_const \<rightleftharpoons> ref_c_ushort.new
 adhoc_overloading store_update_const \<rightleftharpoons> update_fun
 
 micro_c_translate \<open>
-typedef unsigned short uint16_t;
-uint16_t u16_add(uint16_t a, uint16_t b) { return a + b; }
+  typedef unsigned short uint16_t;
+
+  uint16_t u16_add(uint16_t a, uint16_t b) {
+    return a + b;
+  }
 \<close>
 
 thm c_u16_add_def
@@ -692,24 +681,28 @@ ucincl_auto c_u16_add_contract
 
 lemma c_u16_add_spec [crush_specs]:
   shows \<open>\<Gamma>; c_u16_add a b \<Turnstile>\<^sub>F c_u16_add_contract a b\<close>
-  apply (crush_boot f: c_u16_add_def contract: c_u16_add_contract_def)
-  apply (crush_base simp add: c_unsigned_add_def)
-  done
+by (crush_boot f: c_u16_add_def contract: c_u16_add_contract_def)
+  (crush_base simp add: c_unsigned_add_def)
 
 micro_c_translate \<open>
-typedef unsigned long size_t;
-size_t size_add(size_t a, size_t b) { return a + b; }
+  typedef unsigned long size_t;
+
+  size_t size_add(size_t a, size_t b) {
+    return a + b;
+  }
 \<close>
 
 end
 
-section \<open>Void Function Verification\<close>
+section \<open>Void function verification\<close>
 
 context c_uint_verification_ctx
 begin
 
 micro_c_translate \<open>
-void void_write(unsigned int *p, unsigned int v) { *p = v; }
+  void void_write(unsigned int *p, unsigned int v) {
+    *p = v;
+  }
 \<close>
 
 thm c_void_write_def
@@ -725,9 +718,7 @@ ucincl_auto c_void_write_contract
 
 lemma c_void_write_spec [crush_specs]:
   shows \<open>\<Gamma>; c_void_write p v \<Turnstile>\<^sub>F c_void_write_contract p pg old_val v\<close>
-  apply (crush_boot f: c_void_write_def contract: c_void_write_contract_def)
-  apply crush_base
-  done
+by (crush_boot f: c_void_write_def contract: c_void_write_contract_def) crush_base
 
 end
 
@@ -739,17 +730,23 @@ datatype_record c_poly =
 locale c_poly_verification_ctx =
     reference reference_types +
     ref_c_poly: reference_allocatable reference_types _ _ _ _ _ _ _ c_poly_prism
-  for
-    reference_types :: \<open>'s::{sepalg} \<Rightarrow> 'addr \<Rightarrow> 'gv \<Rightarrow> 'abort \<Rightarrow> 'i prompt \<Rightarrow> 'o prompt_output \<Rightarrow> unit\<close>
-    and c_poly_prism :: \<open>('gv, c_poly) prism\<close>
+  for reference_types :: \<open>'s::{sepalg} \<Rightarrow> 'addr \<Rightarrow> 'gv \<Rightarrow> 'abort \<Rightarrow> 'i prompt \<Rightarrow>
+        'o prompt_output \<Rightarrow> unit\<close>
+  and c_poly_prism :: \<open>('gv, c_poly) prism\<close>
 begin
 
 adhoc_overloading store_reference_const \<rightleftharpoons> ref_c_poly.new
 adhoc_overloading store_update_const \<rightleftharpoons> update_fun
 
 micro_c_translate \<open>
-struct poly { int coeffs[256]; };
-int read_coeff(struct poly *p, unsigned int i) { return p->coeffs[i]; }
+
+  struct poly {
+    int coeffs[256];
+  };
+
+  int read_coeff(struct poly *p, unsigned int i) {
+    return p->coeffs[i];
+  }
 \<close>
 
 thm c_read_coeff_def
@@ -759,21 +756,25 @@ definition c_read_coeff_contract ::
      'gv \<Rightarrow> c_poly \<Rightarrow> c_uint \<Rightarrow>
      ('s::{sepalg}, c_int, 'b) function_contract\<close> where
   [crush_contracts]: \<open>c_read_coeff_contract p pg pval i \<equiv>
-    let pre  = p \<mapsto>\<langle>\<top>\<rangle> pg\<down>pval \<star> \<langle>c_idx_to_nat i < length (c_poly_coeffs pval)\<rangle>;
+    let pre  = p \<mapsto>\<langle>\<top>\<rangle> pg\<down>pval \<star>
+               \<langle>c_idx_to_nat i < length (c_poly_coeffs pval)\<rangle>;
         post = \<lambda>r. p \<mapsto>\<langle>\<top>\<rangle> pg\<down>pval \<star>
-                   \<langle>r = c_poly_coeffs pval ! c_idx_to_nat i\<rangle>
+               \<langle>r = c_poly_coeffs pval ! c_idx_to_nat i\<rangle>
      in make_function_contract pre post\<close>
 ucincl_auto c_read_coeff_contract
 
 lemma c_read_coeff_spec [crush_specs]:
   shows \<open>\<Gamma>; c_read_coeff p i \<Turnstile>\<^sub>F c_read_coeff_contract p pg pval i\<close>
-  apply (crush_boot f: c_read_coeff_def contract: c_read_coeff_contract_def)
-  apply crush_base
-  done
+by (crush_boot f: c_read_coeff_def contract: c_read_coeff_contract_def) crush_base
 
 micro_c_translate \<open>
-struct poly { int coeffs[256]; };
-void write_coeff(struct poly *p, unsigned int i, int v) { p->coeffs[i] = v; }
+  struct poly {
+    int coeffs[256];
+  };
+
+  void write_coeff(struct poly *p, unsigned int i, int v) {
+    p->coeffs[i] = v;
+  }
 \<close>
 
 thm c_write_coeff_def
@@ -792,51 +793,51 @@ ucincl_auto c_write_coeff_contract
 
 lemma c_write_coeff_spec [crush_specs]:
   shows \<open>\<Gamma>; c_write_coeff p i v \<Turnstile>\<^sub>F c_write_coeff_contract p pg pval i v\<close>
-  apply (crush_boot f: c_write_coeff_def contract: c_write_coeff_contract_def)
-  apply crush_base
-  done
+by (crush_boot f: c_write_coeff_def contract: c_write_coeff_contract_def) crush_base
 
 end
 
-section \<open>Array Parameter and Local Array Verification\<close>
+section \<open>Array parameter and local array verification\<close>
 
 context c_uint_verification_ctx
 begin
 
 micro_c_translate \<open>
-unsigned int arr_sum(unsigned int arr[], unsigned int i, unsigned int j) {
-  return arr[i] + arr[j];
-}
+
+  unsigned int arr_sum(unsigned int arr[], unsigned int i, unsigned int j) {
+    return arr[i] + arr[j];
+  }
 \<close>
 
 thm c_arr_sum_def
 
 end
 
-section \<open>Byte Buffer Pointer Arithmetic Verification\<close>
+section \<open>Byte buffer pointer arithmetic verification\<close>
 
 locale c_char_verification_ctx =
     reference reference_types +
     ref_c_char: reference_allocatable reference_types _ _ _ _ _ _ _ c_char_prism
-  for
-    reference_types :: \<open>'s::{sepalg} \<Rightarrow> 'addr \<Rightarrow> 'gv \<Rightarrow> 'abort \<Rightarrow> 'i prompt \<Rightarrow> 'o prompt_output \<Rightarrow> unit\<close>
-    and c_char_prism :: \<open>('gv, c_char) prism\<close>
+  for reference_types :: \<open>'s::{sepalg} \<Rightarrow> 'addr \<Rightarrow> 'gv \<Rightarrow> 'abort \<Rightarrow> 'i prompt \<Rightarrow>
+        'o prompt_output \<Rightarrow> unit\<close>
+  and c_char_prism :: \<open>('gv, c_char) prism\<close>
 begin
 
 adhoc_overloading store_reference_const \<rightleftharpoons> ref_c_char.new
 adhoc_overloading store_update_const \<rightleftharpoons> update_fun
 
 micro_c_translate \<open>
-typedef unsigned char uint8_t;
-uint8_t read_byte(uint8_t *buf, unsigned int idx) { return *(buf + idx); }
+  typedef unsigned char uint8_t;
+
+  uint8_t read_byte(uint8_t *buf, unsigned int idx) {
+    return *(buf + idx);
+  }
 \<close>
 
 thm c_read_byte_def
 
-definition c_read_byte_contract ::
-    \<open>('addr, 'gv, c_char list) Global_Store.ref \<Rightarrow>
-     'gv \<Rightarrow> c_char list \<Rightarrow> c_uint \<Rightarrow>
-     ('s::{sepalg}, c_char, 'b) function_contract\<close> where
+definition c_read_byte_contract :: \<open>('addr, 'gv, c_char list) Global_Store.ref \<Rightarrow> 'gv \<Rightarrow>
+     c_char list \<Rightarrow> c_uint \<Rightarrow> ('s::{sepalg}, c_char, 'b) function_contract\<close> where
   [crush_contracts]: \<open>c_read_byte_contract buf bg vs idx \<equiv>
     let pre  = buf \<mapsto>\<langle>\<top>\<rangle> bg\<down>vs \<star> \<langle>c_idx_to_nat idx < length vs\<rangle>;
         post = \<lambda>r. buf \<mapsto>\<langle>\<top>\<rangle> bg\<down>vs \<star> \<langle>r = vs ! c_idx_to_nat idx\<rangle>
@@ -845,10 +846,16 @@ ucincl_auto c_read_byte_contract
 
 lemma c_read_byte_spec [crush_specs]:
   shows \<open>\<Gamma>; c_read_byte buf idx \<Turnstile>\<^sub>F c_read_byte_contract buf bg vs idx\<close>
-  apply (crush_boot f: c_read_byte_def contract: c_read_byte_contract_def)
-  apply crush_base
-  done
+by (crush_boot f: c_read_byte_def contract: c_read_byte_contract_def) crush_base
 
 end
+
+section \<open>Loading C from external files\<close>
+
+text \<open>Test the @{text "micro_c_file"} command which loads C source from a file.\<close>
+
+micro_c_file "test_file.c"
+
+thm c_file_add_def
 
 end
