Micro_C_Examples/C_Struct_Examples.thy
@@ -1,6 +1,3 @@
-(* Copyright Amazon.com, Inc. or its affiliates. All Rights Reserved.
-   SPDX-License-Identifier: MIT *)
-
 theory C_Struct_Examples
   imports
     "Micro_C_Parsing_Frontend.C_To_Core_Translation"
@@ -10,7 +7,7 @@ begin
 
 micro_rust_record c_point
 
-section \<open>C Struct Verification\<close>
+section \<open>C struct verification\<close>
 
 text \<open>
   This theory demonstrates verification of C code operating on structs.
@@ -22,10 +19,10 @@ locale c_struct_verification_ctx =
     reference reference_types +
     ref_c_int: reference_allocatable reference_types _ _ _ _ _ _ _ c_int_prism +
     ref_c_point: reference_allocatable reference_types _ _ _ _ _ _ _ c_point_prism
-  for
-    reference_types :: \<open>'s::{sepalg} \<Rightarrow> 'addr \<Rightarrow> 'gv \<Rightarrow> 'abort \<Rightarrow> 'i prompt \<Rightarrow> 'o prompt_output \<Rightarrow> unit\<close>
-    and c_int_prism :: \<open>('gv, c_int) prism\<close>
-    and c_point_prism :: \<open>('gv, c_point) prism\<close>
+  for reference_types :: \<open>'s::{sepalg} \<Rightarrow> 'addr \<Rightarrow> 'gv \<Rightarrow> 'abort \<Rightarrow> 'i prompt \<Rightarrow>
+        'o prompt_output \<Rightarrow> unit\<close>
+  and c_int_prism :: \<open>('gv, c_int) prism\<close>
+  and c_point_prism :: \<open>('gv, c_point) prism\<close>
 begin
 
 adhoc_overloading store_reference_const \<rightleftharpoons> ref_c_int.new
@@ -33,15 +30,16 @@ adhoc_overloading store_reference_const \<rightleftharpoons> ref_c_point.new
 adhoc_overloading store_update_const \<rightleftharpoons> update_fun
 
 micro_c_translate \<open>
-struct point {
-  int x;
-  int y;
-};
-void swap_coords(struct point *p) {
-  int t = p->x;
-  p->x = p->y;
-  p->y = t;
-}
+  struct point {
+    int x;
+    int y;
+  };
+
+  void swap_coords(struct point *p) {
+    int t = p->x;
+    p->x = p->y;
+    p->y = t;
+  }
 \<close>
 
 thm c_swap_coords_def
@@ -50,16 +48,14 @@ text \<open>
   The contract for swap\_coords: given a reference to a c\_point with value
   @{text pval}, after execution the x and y fields are swapped.
 \<close>
-definition c_swap_coords_contract ::
-    \<open>('addr, 'gv, c_point) Global_Store.ref \<Rightarrow>
-     'gv \<Rightarrow> c_point \<Rightarrow> ('s, 'a, 'b) function_contract\<close> where
+definition c_swap_coords_contract :: \<open>('addr, 'gv, c_point) Global_Store.ref \<Rightarrow> 'gv \<Rightarrow> c_point \<Rightarrow>
+      ('s, 'a, 'b) function_contract\<close> where
   \<open>c_swap_coords_contract pref pg pval \<equiv>
     let pre  = can_alloc_reference \<star>
-               pref \<mapsto>\<langle>\<top>\<rangle> pg\<down>pval in
-    let post = \<lambda> _.
-               can_alloc_reference \<star>
-               pref \<mapsto>\<langle>\<top>\<rangle> (\<lambda>_. make_c_point (c_point_y pval) (c_point_x pval)) \<sqdot> (pg\<down>pval) in
-    make_function_contract pre post\<close>
+               pref \<mapsto>\<langle>\<top>\<rangle> pg\<down>pval;
+        post = \<lambda>_. can_alloc_reference \<star>
+               pref \<mapsto>\<langle>\<top>\<rangle> (\<lambda>_. make_c_point (c_point_y pval) (c_point_x pval)) \<sqdot> (pg\<down>pval)
+     in make_function_contract pre post\<close>
 ucincl_auto c_swap_coords_contract
 
 lemma c_swap_coords_spec:
