Micro_C_Interfaces/Micro_C_Interfaces.thy
@@ -1,6 +1,3 @@
-(* Copyright Amazon.com, Inc. or its affiliates. All Rights Reserved.
-   SPDX-License-Identifier: MIT *)
-
 theory Micro_C_Interfaces
   imports
     "Shallow_Micro_C.Shallow_Micro_C"
