Micro_C_Parsing_Frontend/Micro_C_Parsing_Frontend.thy
@@ -1,6 +1,3 @@
-(* Copyright Amazon.com, Inc. or its affiliates. All Rights Reserved.
-   SPDX-License-Identifier: MIT *)
-
 theory Micro_C_Parsing_Frontend
   imports
     C_To_Core_Translation
