Shallow_Micro_C/C_Arithmetic_Rules.thy
@@ -1,6 +1,3 @@
-(* Copyright Amazon.com, Inc. or its affiliates. All Rights Reserved.
-   SPDX-License-Identifier: MIT *)
-
 theory C_Arithmetic_Rules
   imports
     C_Numeric_Types
@@ -30,514 +27,562 @@ abbreviation c_signed_in_range :: \<open>int \<Rightarrow> nat \<Rightarrow> boo
 subsection \<open>Addition\<close>
 
 lemma wp_c_signed_add [micro_rust_wp_simps]:
-  fixes a b :: \<open>'l::{len} sword\<close>
+    fixes a b :: \<open>'l::{len} sword\<close>
   assumes \<open>\<And>r. ucincl (\<psi> r)\<close>
-  shows \<open>\<W>\<P> \<Gamma> (c_signed_add a b) \<psi> \<rho> \<theta> =
-    (if c_signed_in_range (sint a + sint b) LENGTH('l)
-     then \<psi> (word_of_int (sint a + sint b))
-     else \<theta> (CustomAbort SignedOverflow) \<star> UNIV)\<close>
-  using assms
-  by (simp add: c_signed_add_def c_signed_overflow_def c_abort_def Let_def
-                micro_rust_wp_simps)
+      and \<open>\<And>r. ucincl (\<theta> r)\<close>
+    shows \<open>\<W>\<P> \<Gamma> (c_signed_add a b) \<psi> \<rho> \<theta> =
+             (if c_signed_in_range (sint a + sint b) LENGTH('l) then
+                \<psi> (word_of_int (sint a + sint b))
+              else
+                \<theta> (CustomAbort SignedOverflow))\<close>
+using assms by (auto simp add: c_signed_add_def c_signed_overflow_def c_abort_def Let_def
+  micro_rust_wp_simps asepconj_simp)
 
 lemma wp_c_signed_addI [micro_rust_wp_intros]:
-  fixes a b :: \<open>'l::{len} sword\<close>
-  assumes \<open>c_signed_in_range (sint a + sint b) LENGTH('l)\<close>
-      and \<open>\<phi> \<longlongrightarrow> \<psi> (word_of_int (sint a + sint b)) \<star> \<top>\<close>
-  shows \<open>\<phi> \<longlongrightarrow> \<W>\<P> \<Gamma> (c_signed_add a b) \<psi> \<rho> \<theta>\<close>
+    fixes a b :: \<open>'l::{len} sword\<close>
+  assumes \<open>\<And>r. ucincl (\<psi> r)\<close>
+      and \<open>c_signed_in_range (sint a + sint b) LENGTH('l)\<close>
+      and \<open>\<phi> \<longlongrightarrow> \<psi> (word_of_int (sint a + sint b))\<close>
+    shows \<open>\<phi> \<longlongrightarrow> \<W>\<P> \<Gamma> (c_signed_add a b) \<psi> \<rho> \<theta>\<close>
 proof -
-  from assms(1) have eq: \<open>c_signed_add a b = literal (word_of_int (sint a + sint b))\<close>
+  from assms have eq: \<open>c_signed_add a b = literal (word_of_int (sint a + sint b))\<close>
     by (simp add: c_signed_add_def c_signed_overflow_def Let_def)
-  show ?thesis unfolding eq using assms(2) by (rule wp_literalI)
+  from assms show ?thesis
+    unfolding eq by (auto intro: wp_literalI simp add: asepconj_simp)
 qed
-
 
 subsection \<open>Subtraction\<close>
 
 lemma wp_c_signed_sub [micro_rust_wp_simps]:
-  fixes a b :: \<open>'l::{len} sword\<close>
+    fixes a b :: \<open>'l::{len} sword\<close>
   assumes \<open>\<And>r. ucincl (\<psi> r)\<close>
-  shows \<open>\<W>\<P> \<Gamma> (c_signed_sub a b) \<psi> \<rho> \<theta> =
-    (if c_signed_in_range (sint a - sint b) LENGTH('l)
-     then \<psi> (word_of_int (sint a - sint b))
-     else \<theta> (CustomAbort SignedOverflow) \<star> UNIV)\<close>
-  using assms
-  by (simp add: c_signed_sub_def c_signed_overflow_def c_abort_def Let_def
-                micro_rust_wp_simps)
+      and \<open>\<And>r. ucincl (\<theta> r)\<close>
+    shows \<open>\<W>\<P> \<Gamma> (c_signed_sub a b) \<psi> \<rho> \<theta> =
+            (if c_signed_in_range (sint a - sint b) LENGTH('l) then
+               \<psi> (word_of_int (sint a - sint b))
+             else
+               \<theta> (CustomAbort SignedOverflow))\<close>
+using assms by (simp add: c_signed_sub_def c_signed_overflow_def c_abort_def Let_def
+  micro_rust_wp_simps asepconj_simp)
 
 lemma wp_c_signed_subI [micro_rust_wp_intros]:
-  fixes a b :: \<open>'l::{len} sword\<close>
-  assumes \<open>c_signed_in_range (sint a - sint b) LENGTH('l)\<close>
-      and \<open>\<phi> \<longlongrightarrow> \<psi> (word_of_int (sint a - sint b)) \<star> \<top>\<close>
-  shows \<open>\<phi> \<longlongrightarrow> \<W>\<P> \<Gamma> (c_signed_sub a b) \<psi> \<rho> \<theta>\<close>
+    fixes a b :: \<open>'l::{len} sword\<close>
+  assumes \<open>\<And>r. ucincl (\<psi> r)\<close>
+      and \<open>c_signed_in_range (sint a - sint b) LENGTH('l)\<close>
+      and \<open>\<phi> \<longlongrightarrow> \<psi> (word_of_int (sint a - sint b))\<close>
+    shows \<open>\<phi> \<longlongrightarrow> \<W>\<P> \<Gamma> (c_signed_sub a b) \<psi> \<rho> \<theta>\<close>
 proof -
-  from assms(1) have eq: \<open>c_signed_sub a b = literal (word_of_int (sint a - sint b))\<close>
+  from assms have eq: \<open>c_signed_sub a b = literal (word_of_int (sint a - sint b))\<close>
     by (simp add: c_signed_sub_def c_signed_overflow_def Let_def)
-  show ?thesis unfolding eq using assms(2) by (rule wp_literalI)
+  from assms show ?thesis
+    unfolding eq by (auto intro: wp_literalI simp add: asepconj_simp)
 qed
 
 subsection \<open>Multiplication\<close>
 
 lemma wp_c_signed_mul [micro_rust_wp_simps]:
-  fixes a b :: \<open>'l::{len} sword\<close>
+    fixes a b :: \<open>'l::{len} sword\<close>
   assumes \<open>\<And>r. ucincl (\<psi> r)\<close>
-  shows \<open>\<W>\<P> \<Gamma> (c_signed_mul a b) \<psi> \<rho> \<theta> =
-    (if c_signed_in_range (sint a * sint b) LENGTH('l)
-     then \<psi> (word_of_int (sint a * sint b))
-     else \<theta> (CustomAbort SignedOverflow) \<star> UNIV)\<close>
-  using assms
-  by (simp add: c_signed_mul_def c_signed_overflow_def c_abort_def Let_def
-                micro_rust_wp_simps)
+      and \<open>\<And>r. ucincl (\<theta> r)\<close>
+    shows \<open>\<W>\<P> \<Gamma> (c_signed_mul a b) \<psi> \<rho> \<theta> =
+             (if c_signed_in_range (sint a * sint b) LENGTH('l) then
+                \<psi> (word_of_int (sint a * sint b))
+              else
+                \<theta> (CustomAbort SignedOverflow))\<close>
+using assms by (simp add: c_signed_mul_def c_signed_overflow_def c_abort_def Let_def
+  micro_rust_wp_simps asepconj_simp)
 
 lemma wp_c_signed_mulI [micro_rust_wp_intros]:
-  fixes a b :: \<open>'l::{len} sword\<close>
-  assumes \<open>c_signed_in_range (sint a * sint b) LENGTH('l)\<close>
-      and \<open>\<phi> \<longlongrightarrow> \<psi> (word_of_int (sint a * sint b)) \<star> \<top>\<close>
-  shows \<open>\<phi> \<longlongrightarrow> \<W>\<P> \<Gamma> (c_signed_mul a b) \<psi> \<rho> \<theta>\<close>
+    fixes a b :: \<open>'l::{len} sword\<close>
+  assumes \<open>\<And>r. ucincl (\<psi> r)\<close>
+      and \<open>c_signed_in_range (sint a * sint b) LENGTH('l)\<close>
+      and \<open>\<phi> \<longlongrightarrow> \<psi> (word_of_int (sint a * sint b))\<close>
+    shows \<open>\<phi> \<longlongrightarrow> \<W>\<P> \<Gamma> (c_signed_mul a b) \<psi> \<rho> \<theta>\<close>
 proof -
-  from assms(1) have eq: \<open>c_signed_mul a b = literal (word_of_int (sint a * sint b))\<close>
+  from assms have eq: \<open>c_signed_mul a b = literal (word_of_int (sint a * sint b))\<close>
     by (simp add: c_signed_mul_def c_signed_overflow_def Let_def)
-  show ?thesis unfolding eq using assms(2) by (rule wp_literalI)
+  from assms show ?thesis
+    unfolding eq by (auto intro: wp_literalI simp add: asepconj_simp)
 qed
 
 subsection \<open>Division\<close>
 
 lemma wp_c_signed_div [micro_rust_wp_simps]:
-  fixes a b :: \<open>'l::{len} sword\<close>
+    fixes a b :: \<open>'l::{len} sword\<close>
   assumes \<open>\<And>r. ucincl (\<psi> r)\<close>
-  shows \<open>\<W>\<P> \<Gamma> (c_signed_div a b) \<psi> \<rho> \<theta> =
-    (if b = 0 then \<theta> (CustomAbort DivisionByZero) \<star> UNIV
-     else if c_signed_in_range (sint a div sint b) LENGTH('l)
-     then \<psi> (word_of_int (sint a div sint b))
-     else \<theta> (CustomAbort SignedOverflow) \<star> UNIV)\<close>
-  using assms
-  by (simp add: c_signed_div_def c_signed_overflow_def c_abort_def c_division_by_zero_def Let_def
-                micro_rust_wp_simps)
+      and \<open>\<And>r. ucincl (\<theta> r)\<close>
+    shows \<open>\<W>\<P> \<Gamma> (c_signed_div a b) \<psi> \<rho> \<theta> =
+             (if b = 0 then
+                \<theta> (CustomAbort DivisionByZero)
+              else if c_signed_in_range (sint a div sint b) LENGTH('l) then
+                \<psi> (word_of_int (sint a div sint b))
+              else
+                \<theta> (CustomAbort SignedOverflow))\<close>
+using assms by (simp add: c_signed_div_def c_signed_overflow_def c_abort_def c_division_by_zero_def
+  Let_def micro_rust_wp_simps asepconj_simp)
 
 lemma wp_c_signed_divI [micro_rust_wp_intros]:
-  fixes a b :: \<open>'l::{len} sword\<close>
-  assumes \<open>b \<noteq> 0\<close>
+    fixes a b :: \<open>'l::{len} sword\<close>
+  assumes \<open>\<And>r. ucincl (\<psi> r)\<close>
+      and \<open>b \<noteq> 0\<close>
       and \<open>c_signed_in_range (sint a div sint b) LENGTH('l)\<close>
-      and \<open>\<phi> \<longlongrightarrow> \<psi> (word_of_int (sint a div sint b)) \<star> \<top>\<close>
-  shows \<open>\<phi> \<longlongrightarrow> \<W>\<P> \<Gamma> (c_signed_div a b) \<psi> \<rho> \<theta>\<close>
+      and \<open>\<phi> \<longlongrightarrow> \<psi> (word_of_int (sint a div sint b))\<close>
+    shows \<open>\<phi> \<longlongrightarrow> \<W>\<P> \<Gamma> (c_signed_div a b) \<psi> \<rho> \<theta>\<close>
 proof -
-  from assms(1,2) have eq: \<open>c_signed_div a b = literal (word_of_int (sint a div sint b))\<close>
+  from assms have eq: \<open>c_signed_div a b = literal (word_of_int (sint a div sint b))\<close>
     by (simp add: c_signed_div_def c_signed_overflow_def c_division_by_zero_def Let_def)
-  show ?thesis unfolding eq using assms(3) by (rule wp_literalI)
+  from assms this show ?thesis
+    unfolding eq by (auto intro: wp_literalI simp add: asepconj_simp)
 qed
 
 subsection \<open>Modulo\<close>
 
 lemma wp_c_signed_mod [micro_rust_wp_simps]:
-  fixes a b :: \<open>'l::{len} sword\<close>
+    fixes a b :: \<open>'l::{len} sword\<close>
   assumes \<open>\<And>r. ucincl (\<psi> r)\<close>
-  shows \<open>\<W>\<P> \<Gamma> (c_signed_mod a b) \<psi> \<rho> \<theta> =
-    (if b = 0 then \<theta> (CustomAbort DivisionByZero) \<star> UNIV
-     else \<psi> (word_of_int (sint a mod sint b)))\<close>
-  using assms
-  by (simp add: c_signed_mod_def c_abort_def c_division_by_zero_def Let_def
-                micro_rust_wp_simps)
+      and \<open>\<And>r. ucincl (\<theta> r)\<close>
+    shows \<open>\<W>\<P> \<Gamma> (c_signed_mod a b) \<psi> \<rho> \<theta> =
+            (if b = 0 then
+               \<theta> (CustomAbort DivisionByZero)
+             else
+               \<psi> (word_of_int (sint a mod sint b)))\<close>
+using assms by (simp add: c_signed_mod_def c_abort_def c_division_by_zero_def Let_def
+  micro_rust_wp_simps asepconj_simp)
 
 lemma wp_c_signed_modI [micro_rust_wp_intros]:
-  fixes a b :: \<open>'l::{len} sword\<close>
-  assumes \<open>b \<noteq> 0\<close>
-      and \<open>\<phi> \<longlongrightarrow> \<psi> (word_of_int (sint a mod sint b)) \<star> \<top>\<close>
-  shows \<open>\<phi> \<longlongrightarrow> \<W>\<P> \<Gamma> (c_signed_mod a b) \<psi> \<rho> \<theta>\<close>
+    fixes a b :: \<open>'l::{len} sword\<close>
+  assumes \<open>\<And>r. ucincl (\<psi> r)\<close>
+      and \<open>b \<noteq> 0\<close>
+      and \<open>\<phi> \<longlongrightarrow> \<psi> (word_of_int (sint a mod sint b))\<close>
+    shows \<open>\<phi> \<longlongrightarrow> \<W>\<P> \<Gamma> (c_signed_mod a b) \<psi> \<rho> \<theta>\<close>
 proof -
-  from assms(1) have eq: \<open>c_signed_mod a b = literal (word_of_int (sint a mod sint b))\<close>
+  from assms have eq: \<open>c_signed_mod a b = literal (word_of_int (sint a mod sint b))\<close>
     by (simp add: c_signed_mod_def c_division_by_zero_def Let_def)
-  show ?thesis unfolding eq using assms(2) by (rule wp_literalI)
+  from this assms show ?thesis
+    unfolding eq by (auto intro: wp_literalI simp add: asepconj_simp)
 qed
 
-subsection \<open>Comparison Operations\<close>
+subsection \<open>Comparison operations\<close>
 
 text \<open>Comparisons never overflow --- they always succeed.\<close>
 
 lemma wp_c_signed_less [micro_rust_wp_simps]:
-  fixes a b :: \<open>'l::{len} sword\<close>
+    fixes a b :: \<open>'l::{len} sword\<close>
   assumes \<open>\<And>r. ucincl (\<psi> r)\<close>
-  shows \<open>\<W>\<P> \<Gamma> (c_signed_less a b) \<psi> \<rho> \<theta> = \<psi> (sint a < sint b)\<close>
-  using assms
-  by (simp add: c_signed_less_def micro_rust_wp_simps)
+    shows \<open>\<W>\<P> \<Gamma> (c_signed_less a b) \<psi> \<rho> \<theta> = \<psi> (sint a < sint b)\<close>
+using assms by (simp add: c_signed_less_def micro_rust_wp_simps)
 
 lemma wp_c_signed_lessI [micro_rust_wp_intros]:
-  fixes a b :: \<open>'l::{len} sword\<close>
-  assumes \<open>\<phi> \<longlongrightarrow> \<psi> (sint a < sint b) \<star> \<top>\<close>
-  shows \<open>\<phi> \<longlongrightarrow> \<W>\<P> \<Gamma> (c_signed_less a b) \<psi> \<rho> \<theta>\<close>
-  using assms by (simp add: c_signed_less_def wp_literalI)
+    fixes a b :: \<open>'l::{len} sword\<close>
+  assumes \<open>\<And>r. ucincl (\<psi> r)\<close>
+      and \<open>\<phi> \<longlongrightarrow> \<psi> (sint a < sint b)\<close>
+    shows \<open>\<phi> \<longlongrightarrow> \<W>\<P> \<Gamma> (c_signed_less a b) \<psi> \<rho> \<theta>\<close>
+using assms by (simp add: c_signed_less_def wp_literalI asepconj_simp)
 
 lemma wp_c_signed_le [micro_rust_wp_simps]:
-  fixes a b :: \<open>'l::{len} sword\<close>
+    fixes a b :: \<open>'l::{len} sword\<close>
   assumes \<open>\<And>r. ucincl (\<psi> r)\<close>
-  shows \<open>\<W>\<P> \<Gamma> (c_signed_le a b) \<psi> \<rho> \<theta> = \<psi> (sint a \<le> sint b)\<close>
-  using assms
-  by (simp add: c_signed_le_def micro_rust_wp_simps)
+    shows \<open>\<W>\<P> \<Gamma> (c_signed_le a b) \<psi> \<rho> \<theta> = \<psi> (sint a \<le> sint b)\<close>
+using assms by (simp add: c_signed_le_def micro_rust_wp_simps)
 
 lemma wp_c_signed_leI [micro_rust_wp_intros]:
-  fixes a b :: \<open>'l::{len} sword\<close>
-  assumes \<open>\<phi> \<longlongrightarrow> \<psi> (sint a \<le> sint b) \<star> \<top>\<close>
-  shows \<open>\<phi> \<longlongrightarrow> \<W>\<P> \<Gamma> (c_signed_le a b) \<psi> \<rho> \<theta>\<close>
-  using assms by (simp add: c_signed_le_def wp_literalI)
+    fixes a b :: \<open>'l::{len} sword\<close>
+  assumes \<open>\<And>r. ucincl (\<psi> r)\<close>
+      and \<open>\<phi> \<longlongrightarrow> \<psi> (sint a \<le> sint b)\<close>
+    shows \<open>\<phi> \<longlongrightarrow> \<W>\<P> \<Gamma> (c_signed_le a b) \<psi> \<rho> \<theta>\<close>
+using assms by (simp add: c_signed_le_def wp_literalI asepconj_simp)
 
 lemma wp_c_signed_eq [micro_rust_wp_simps]:
-  fixes a b :: \<open>'l::{len} sword\<close>
+    fixes a b :: \<open>'l::{len} sword\<close>
   assumes \<open>\<And>r. ucincl (\<psi> r)\<close>
-  shows \<open>\<W>\<P> \<Gamma> (c_signed_eq a b) \<psi> \<rho> \<theta> = \<psi> (a = b)\<close>
-  using assms
-  by (simp add: c_signed_eq_def micro_rust_wp_simps)
+    shows \<open>\<W>\<P> \<Gamma> (c_signed_eq a b) \<psi> \<rho> \<theta> = \<psi> (a = b)\<close>
+using assms by (simp add: c_signed_eq_def micro_rust_wp_simps)
 
 lemma wp_c_signed_eqI [micro_rust_wp_intros]:
-  fixes a b :: \<open>'l::{len} sword\<close>
-  assumes \<open>\<phi> \<longlongrightarrow> \<psi> (a = b) \<star> \<top>\<close>
-  shows \<open>\<phi> \<longlongrightarrow> \<W>\<P> \<Gamma> (c_signed_eq a b) \<psi> \<rho> \<theta>\<close>
-  using assms by (simp add: c_signed_eq_def wp_literalI)
+    fixes a b :: \<open>'l::{len} sword\<close>
+  assumes \<open>\<And>r. ucincl (\<psi> r)\<close>
+      and \<open>\<phi> \<longlongrightarrow> \<psi> (a = b)\<close>
+    shows \<open>\<phi> \<longlongrightarrow> \<W>\<P> \<Gamma> (c_signed_eq a b) \<psi> \<rho> \<theta>\<close>
+using assms by (simp add: c_signed_eq_def wp_literalI asepconj_simp)
 
 lemma wp_c_signed_neq [micro_rust_wp_simps]:
-  fixes a b :: \<open>'l::{len} sword\<close>
+    fixes a b :: \<open>'l::{len} sword\<close>
   assumes \<open>\<And>r. ucincl (\<psi> r)\<close>
-  shows \<open>\<W>\<P> \<Gamma> (c_signed_neq a b) \<psi> \<rho> \<theta> = \<psi> (a \<noteq> b)\<close>
-  using assms
-  by (simp add: c_signed_neq_def micro_rust_wp_simps)
+    shows \<open>\<W>\<P> \<Gamma> (c_signed_neq a b) \<psi> \<rho> \<theta> = \<psi> (a \<noteq> b)\<close>
+using assms by (simp add: c_signed_neq_def micro_rust_wp_simps)
 
 lemma wp_c_signed_neqI [micro_rust_wp_intros]:
-  fixes a b :: \<open>'l::{len} sword\<close>
-  assumes \<open>\<phi> \<longlongrightarrow> \<psi> (a \<noteq> b) \<star> \<top>\<close>
-  shows \<open>\<phi> \<longlongrightarrow> \<W>\<P> \<Gamma> (c_signed_neq a b) \<psi> \<rho> \<theta>\<close>
-  using assms by (simp add: c_signed_neq_def wp_literalI)
+    fixes a b :: \<open>'l::{len} sword\<close>
+  assumes \<open>\<And>r. ucincl (\<psi> r)\<close>
+      and \<open>\<phi> \<longlongrightarrow> \<psi> (a \<noteq> b)\<close>
+    shows \<open>\<phi> \<longlongrightarrow> \<W>\<P> \<Gamma> (c_signed_neq a b) \<psi> \<rho> \<theta>\<close>
+using assms by (simp add: c_signed_neq_def wp_literalI asepconj_simp)
 
-subsection \<open>Unsigned Addition\<close>
+subsection \<open>Unsigned addition\<close>
 
 lemma wp_c_unsigned_add [micro_rust_wp_simps]:
-  fixes a b :: \<open>'l::{len} word\<close>
+    fixes a b :: \<open>'l::{len} word\<close>
   assumes \<open>\<And>r. ucincl (\<psi> r)\<close>
-  shows \<open>\<W>\<P> \<Gamma> (c_unsigned_add a b) \<psi> \<rho> \<theta> = \<psi> (a + b)\<close>
-  using assms
-  by (simp add: c_unsigned_add_def micro_rust_wp_simps)
+    shows \<open>\<W>\<P> \<Gamma> (c_unsigned_add a b) \<psi> \<rho> \<theta> = \<psi> (a + b)\<close>
+using assms by (simp add: c_unsigned_add_def micro_rust_wp_simps)
 
 lemma wp_c_unsigned_addI [micro_rust_wp_intros]:
-  fixes a b :: \<open>'l::{len} word\<close>
-  assumes \<open>\<phi> \<longlongrightarrow> \<psi> (a + b) \<star> \<top>\<close>
-  shows \<open>\<phi> \<longlongrightarrow> \<W>\<P> \<Gamma> (c_unsigned_add a b) \<psi> \<rho> \<theta>\<close>
-  using assms by (simp add: c_unsigned_add_def wp_literalI)
+    fixes a b :: \<open>'l::{len} word\<close>
+  assumes \<open>\<And>r. ucincl (\<psi> r)\<close>
+      and \<open>\<phi> \<longlongrightarrow> \<psi> (a + b)\<close>
+    shows \<open>\<phi> \<longlongrightarrow> \<W>\<P> \<Gamma> (c_unsigned_add a b) \<psi> \<rho> \<theta>\<close>
+using assms by (simp add: c_unsigned_add_def wp_literalI asepconj_simp)
 
 subsection \<open>Unsigned Subtraction\<close>
 
 lemma wp_c_unsigned_sub [micro_rust_wp_simps]:
-  fixes a b :: \<open>'l::{len} word\<close>
+    fixes a b :: \<open>'l::{len} word\<close>
   assumes \<open>\<And>r. ucincl (\<psi> r)\<close>
-  shows \<open>\<W>\<P> \<Gamma> (c_unsigned_sub a b) \<psi> \<rho> \<theta> = \<psi> (a - b)\<close>
-  using assms
-  by (simp add: c_unsigned_sub_def micro_rust_wp_simps)
+    shows \<open>\<W>\<P> \<Gamma> (c_unsigned_sub a b) \<psi> \<rho> \<theta> = \<psi> (a - b)\<close>
+using assms by (simp add: c_unsigned_sub_def micro_rust_wp_simps)
 
 lemma wp_c_unsigned_subI [micro_rust_wp_intros]:
-  fixes a b :: \<open>'l::{len} word\<close>
-  assumes \<open>\<phi> \<longlongrightarrow> \<psi> (a - b) \<star> \<top>\<close>
-  shows \<open>\<phi> \<longlongrightarrow> \<W>\<P> \<Gamma> (c_unsigned_sub a b) \<psi> \<rho> \<theta>\<close>
-  using assms by (simp add: c_unsigned_sub_def wp_literalI)
+    fixes a b :: \<open>'l::{len} word\<close>
+  assumes \<open>\<And>r. ucincl (\<psi> r)\<close>
+      and \<open>\<phi> \<longlongrightarrow> \<psi> (a - b)\<close>
+    shows \<open>\<phi> \<longlongrightarrow> \<W>\<P> \<Gamma> (c_unsigned_sub a b) \<psi> \<rho> \<theta>\<close>
+using assms by (simp add: c_unsigned_sub_def wp_literalI asepconj_simp)
 
 subsection \<open>Unsigned Multiplication\<close>
 
 lemma wp_c_unsigned_mul [micro_rust_wp_simps]:
-  fixes a b :: \<open>'l::{len} word\<close>
+    fixes a b :: \<open>'l::{len} word\<close>
   assumes \<open>\<And>r. ucincl (\<psi> r)\<close>
-  shows \<open>\<W>\<P> \<Gamma> (c_unsigned_mul a b) \<psi> \<rho> \<theta> = \<psi> (a * b)\<close>
-  using assms
-  by (simp add: c_unsigned_mul_def micro_rust_wp_simps)
+    shows \<open>\<W>\<P> \<Gamma> (c_unsigned_mul a b) \<psi> \<rho> \<theta> = \<psi> (a * b)\<close>
+using assms by (simp add: c_unsigned_mul_def micro_rust_wp_simps)
 
 lemma wp_c_unsigned_mulI [micro_rust_wp_intros]:
-  fixes a b :: \<open>'l::{len} word\<close>
-  assumes \<open>\<phi> \<longlongrightarrow> \<psi> (a * b) \<star> \<top>\<close>
-  shows \<open>\<phi> \<longlongrightarrow> \<W>\<P> \<Gamma> (c_unsigned_mul a b) \<psi> \<rho> \<theta>\<close>
-  using assms by (simp add: c_unsigned_mul_def wp_literalI)
+    fixes a b :: \<open>'l::{len} word\<close>
+  assumes \<open>\<And>r. ucincl (\<psi> r)\<close>
+      and \<open>\<phi> \<longlongrightarrow> \<psi> (a * b)\<close>
+    shows \<open>\<phi> \<longlongrightarrow> \<W>\<P> \<Gamma> (c_unsigned_mul a b) \<psi> \<rho> \<theta>\<close>
+using assms by (simp add: c_unsigned_mul_def wp_literalI asepconj_simp)
 
 subsection \<open>Unsigned Comparison Operations\<close>
 
 lemma wp_c_unsigned_less [micro_rust_wp_simps]:
-  fixes a b :: \<open>'l::{len} word\<close>
+    fixes a b :: \<open>'l::{len} word\<close>
   assumes \<open>\<And>r. ucincl (\<psi> r)\<close>
-  shows \<open>\<W>\<P> \<Gamma> (c_unsigned_less a b) \<psi> \<rho> \<theta> = \<psi> (a < b)\<close>
-  using assms
-  by (simp add: c_unsigned_less_def micro_rust_wp_simps)
+    shows \<open>\<W>\<P> \<Gamma> (c_unsigned_less a b) \<psi> \<rho> \<theta> = \<psi> (a < b)\<close>
+using assms by (simp add: c_unsigned_less_def micro_rust_wp_simps)
 
 lemma wp_c_unsigned_lessI [micro_rust_wp_intros]:
-  fixes a b :: \<open>'l::{len} word\<close>
-  assumes \<open>\<phi> \<longlongrightarrow> \<psi> (a < b) \<star> \<top>\<close>
-  shows \<open>\<phi> \<longlongrightarrow> \<W>\<P> \<Gamma> (c_unsigned_less a b) \<psi> \<rho> \<theta>\<close>
-  using assms by (simp add: c_unsigned_less_def wp_literalI)
+    fixes a b :: \<open>'l::{len} word\<close>
+  assumes \<open>\<And>r. ucincl (\<psi> r)\<close>
+      and \<open>\<phi> \<longlongrightarrow> \<psi> (a < b)\<close>
+    shows \<open>\<phi> \<longlongrightarrow> \<W>\<P> \<Gamma> (c_unsigned_less a b) \<psi> \<rho> \<theta>\<close>
+using assms by (simp add: c_unsigned_less_def wp_literalI asepconj_simp)
 
 lemma wp_c_unsigned_le [micro_rust_wp_simps]:
-  fixes a b :: \<open>'l::{len} word\<close>
+    fixes a b :: \<open>'l::{len} word\<close>
   assumes \<open>\<And>r. ucincl (\<psi> r)\<close>
-  shows \<open>\<W>\<P> \<Gamma> (c_unsigned_le a b) \<psi> \<rho> \<theta> = \<psi> (a \<le> b)\<close>
-  using assms
-  by (simp add: c_unsigned_le_def micro_rust_wp_simps)
+    shows \<open>\<W>\<P> \<Gamma> (c_unsigned_le a b) \<psi> \<rho> \<theta> = \<psi> (a \<le> b)\<close>
+using assms by (simp add: c_unsigned_le_def micro_rust_wp_simps)
 
 lemma wp_c_unsigned_leI [micro_rust_wp_intros]:
-  fixes a b :: \<open>'l::{len} word\<close>
-  assumes \<open>\<phi> \<longlongrightarrow> \<psi> (a \<le> b) \<star> \<top>\<close>
-  shows \<open>\<phi> \<longlongrightarrow> \<W>\<P> \<Gamma> (c_unsigned_le a b) \<psi> \<rho> \<theta>\<close>
-  using assms by (simp add: c_unsigned_le_def wp_literalI)
+    fixes a b :: \<open>'l::{len} word\<close>
+  assumes \<open>\<And>r. ucincl (\<psi> r)\<close>
+      and \<open>\<phi> \<longlongrightarrow> \<psi> (a \<le> b)\<close>
+    shows \<open>\<phi> \<longlongrightarrow> \<W>\<P> \<Gamma> (c_unsigned_le a b) \<psi> \<rho> \<theta>\<close>
+using assms by (simp add: c_unsigned_le_def wp_literalI asepconj_simp)
 
 lemma wp_c_unsigned_eq [micro_rust_wp_simps]:
-  fixes a b :: \<open>'l::{len} word\<close>
+    fixes a b :: \<open>'l::{len} word\<close>
   assumes \<open>\<And>r. ucincl (\<psi> r)\<close>
-  shows \<open>\<W>\<P> \<Gamma> (c_unsigned_eq a b) \<psi> \<rho> \<theta> = \<psi> (a = b)\<close>
-  using assms
-  by (simp add: c_unsigned_eq_def micro_rust_wp_simps)
+    shows \<open>\<W>\<P> \<Gamma> (c_unsigned_eq a b) \<psi> \<rho> \<theta> = \<psi> (a = b)\<close>
+using assms by (simp add: c_unsigned_eq_def micro_rust_wp_simps)
 
 lemma wp_c_unsigned_eqI [micro_rust_wp_intros]:
-  fixes a b :: \<open>'l::{len} word\<close>
-  assumes \<open>\<phi> \<longlongrightarrow> \<psi> (a = b) \<star> \<top>\<close>
-  shows \<open>\<phi> \<longlongrightarrow> \<W>\<P> \<Gamma> (c_unsigned_eq a b) \<psi> \<rho> \<theta>\<close>
-  using assms by (simp add: c_unsigned_eq_def wp_literalI)
+    fixes a b :: \<open>'l::{len} word\<close>
+  assumes \<open>\<And>r. ucincl (\<psi> r)\<close>
+      and \<open>\<phi> \<longlongrightarrow> \<psi> (a = b)\<close>
+    shows \<open>\<phi> \<longlongrightarrow> \<W>\<P> \<Gamma> (c_unsigned_eq a b) \<psi> \<rho> \<theta>\<close>
+using assms by (simp add: c_unsigned_eq_def wp_literalI asepconj_simp)
 
 lemma wp_c_unsigned_neq [micro_rust_wp_simps]:
-  fixes a b :: \<open>'l::{len} word\<close>
+    fixes a b :: \<open>'l::{len} word\<close>
   assumes \<open>\<And>r. ucincl (\<psi> r)\<close>
-  shows \<open>\<W>\<P> \<Gamma> (c_unsigned_neq a b) \<psi> \<rho> \<theta> = \<psi> (a \<noteq> b)\<close>
-  using assms
-  by (simp add: c_unsigned_neq_def micro_rust_wp_simps)
+    shows \<open>\<W>\<P> \<Gamma> (c_unsigned_neq a b) \<psi> \<rho> \<theta> = \<psi> (a \<noteq> b)\<close>
+using assms by (simp add: c_unsigned_neq_def micro_rust_wp_simps)
 
 lemma wp_c_unsigned_neqI [micro_rust_wp_intros]:
-  fixes a b :: \<open>'l::{len} word\<close>
-  assumes \<open>\<phi> \<longlongrightarrow> \<psi> (a \<noteq> b) \<star> \<top>\<close>
-  shows \<open>\<phi> \<longlongrightarrow> \<W>\<P> \<Gamma> (c_unsigned_neq a b) \<psi> \<rho> \<theta>\<close>
-  using assms by (simp add: c_unsigned_neq_def wp_literalI)
+    fixes a b :: \<open>'l::{len} word\<close>
+  assumes \<open>\<And>r. ucincl (\<psi> r)\<close>
+      and \<open>\<phi> \<longlongrightarrow> \<psi> (a \<noteq> b)\<close>
+    shows \<open>\<phi> \<longlongrightarrow> \<W>\<P> \<Gamma> (c_unsigned_neq a b) \<psi> \<rho> \<theta>\<close>
+using assms by (simp add: c_unsigned_neq_def wp_literalI asepconj_simp)
 
-subsection \<open>Signed Bitwise Operations\<close>
+subsection \<open>Signed bitwise operations\<close>
 
 lemma wp_c_signed_and [micro_rust_wp_simps]:
-  fixes a b :: \<open>'l::{len} sword\<close>
+    fixes a b :: \<open>'l::{len} sword\<close>
   assumes \<open>\<And>r. ucincl (\<psi> r)\<close>
-  shows \<open>\<W>\<P> \<Gamma> (c_signed_and a b) \<psi> \<rho> \<theta> = \<psi> (a AND b)\<close>
-  using assms by (simp add: c_signed_and_def micro_rust_wp_simps)
+    shows \<open>\<W>\<P> \<Gamma> (c_signed_and a b) \<psi> \<rho> \<theta> = \<psi> (a AND b)\<close>
+using assms by (simp add: c_signed_and_def micro_rust_wp_simps)
 
 lemma wp_c_signed_andI [micro_rust_wp_intros]:
-  fixes a b :: \<open>'l::{len} sword\<close>
-  assumes \<open>\<phi> \<longlongrightarrow> \<psi> (a AND b) \<star> \<top>\<close>
-  shows \<open>\<phi> \<longlongrightarrow> \<W>\<P> \<Gamma> (c_signed_and a b) \<psi> \<rho> \<theta>\<close>
-  using assms by (simp add: c_signed_and_def wp_literalI)
+    fixes a b :: \<open>'l::{len} sword\<close>
+  assumes \<open>\<And>r. ucincl (\<psi> r)\<close>
+      and \<open>\<phi> \<longlongrightarrow> \<psi> (a AND b)\<close>
+    shows \<open>\<phi> \<longlongrightarrow> \<W>\<P> \<Gamma> (c_signed_and a b) \<psi> \<rho> \<theta>\<close>
+using assms by (simp add: c_signed_and_def wp_literalI asepconj_simp)
 
 lemma wp_c_signed_or [micro_rust_wp_simps]:
-  fixes a b :: \<open>'l::{len} sword\<close>
+    fixes a b :: \<open>'l::{len} sword\<close>
   assumes \<open>\<And>r. ucincl (\<psi> r)\<close>
-  shows \<open>\<W>\<P> \<Gamma> (c_signed_or a b) \<psi> \<rho> \<theta> = \<psi> (a OR b)\<close>
-  using assms by (simp add: c_signed_or_def micro_rust_wp_simps)
+    shows \<open>\<W>\<P> \<Gamma> (c_signed_or a b) \<psi> \<rho> \<theta> = \<psi> (a OR b)\<close>
+using assms by (simp add: c_signed_or_def micro_rust_wp_simps)
 
 lemma wp_c_signed_orI [micro_rust_wp_intros]:
-  fixes a b :: \<open>'l::{len} sword\<close>
-  assumes \<open>\<phi> \<longlongrightarrow> \<psi> (a OR b) \<star> \<top>\<close>
-  shows \<open>\<phi> \<longlongrightarrow> \<W>\<P> \<Gamma> (c_signed_or a b) \<psi> \<rho> \<theta>\<close>
-  using assms by (simp add: c_signed_or_def wp_literalI)
+    fixes a b :: \<open>'l::{len} sword\<close>
+  assumes \<open>\<And>r. ucincl (\<psi> r)\<close>
+      and \<open>\<phi> \<longlongrightarrow> \<psi> (a OR b)\<close>
+    shows \<open>\<phi> \<longlongrightarrow> \<W>\<P> \<Gamma> (c_signed_or a b) \<psi> \<rho> \<theta>\<close>
+using assms by (simp add: c_signed_or_def wp_literalI asepconj_simp)
 
 lemma wp_c_signed_xor [micro_rust_wp_simps]:
-  fixes a b :: \<open>'l::{len} sword\<close>
+    fixes a b :: \<open>'l::{len} sword\<close>
   assumes \<open>\<And>r. ucincl (\<psi> r)\<close>
-  shows \<open>\<W>\<P> \<Gamma> (c_signed_xor a b) \<psi> \<rho> \<theta> = \<psi> (a XOR b)\<close>
-  using assms by (simp add: c_signed_xor_def micro_rust_wp_simps)
+    shows \<open>\<W>\<P> \<Gamma> (c_signed_xor a b) \<psi> \<rho> \<theta> = \<psi> (a XOR b)\<close>
+using assms by (simp add: c_signed_xor_def micro_rust_wp_simps)
 
 lemma wp_c_signed_xorI [micro_rust_wp_intros]:
-  fixes a b :: \<open>'l::{len} sword\<close>
-  assumes \<open>\<phi> \<longlongrightarrow> \<psi> (a XOR b) \<star> \<top>\<close>
-  shows \<open>\<phi> \<longlongrightarrow> \<W>\<P> \<Gamma> (c_signed_xor a b) \<psi> \<rho> \<theta>\<close>
-  using assms by (simp add: c_signed_xor_def wp_literalI)
+    fixes a b :: \<open>'l::{len} sword\<close>
+  assumes \<open>\<And>r. ucincl (\<psi> r)\<close>
+      and \<open>\<phi> \<longlongrightarrow> \<psi> (a XOR b)\<close>
+    shows \<open>\<phi> \<longlongrightarrow> \<W>\<P> \<Gamma> (c_signed_xor a b) \<psi> \<rho> \<theta>\<close>
+using assms by (simp add: c_signed_xor_def wp_literalI asepconj_simp)
 
 lemma wp_c_signed_not [micro_rust_wp_simps]:
-  fixes a :: \<open>'l::{len} sword\<close>
+    fixes a :: \<open>'l::{len} sword\<close>
   assumes \<open>\<And>r. ucincl (\<psi> r)\<close>
-  shows \<open>\<W>\<P> \<Gamma> (c_signed_not a) \<psi> \<rho> \<theta> = \<psi> (NOT a)\<close>
-  using assms by (simp add: c_signed_not_def micro_rust_wp_simps)
+    shows \<open>\<W>\<P> \<Gamma> (c_signed_not a) \<psi> \<rho> \<theta> = \<psi> (NOT a)\<close>
+using assms by (simp add: c_signed_not_def micro_rust_wp_simps)
 
 lemma wp_c_signed_notI [micro_rust_wp_intros]:
-  fixes a :: \<open>'l::{len} sword\<close>
-  assumes \<open>\<phi> \<longlongrightarrow> \<psi> (NOT a) \<star> \<top>\<close>
-  shows \<open>\<phi> \<longlongrightarrow> \<W>\<P> \<Gamma> (c_signed_not a) \<psi> \<rho> \<theta>\<close>
-  using assms by (simp add: c_signed_not_def wp_literalI)
+    fixes a :: \<open>'l::{len} sword\<close>
+  assumes \<open>\<And>r. ucincl (\<psi> r)\<close>
+      and \<open>\<phi> \<longlongrightarrow> \<psi> (NOT a)\<close>
+    shows \<open>\<phi> \<longlongrightarrow> \<W>\<P> \<Gamma> (c_signed_not a) \<psi> \<rho> \<theta>\<close>
+using assms by (simp add: c_signed_not_def wp_literalI asepconj_simp)
 
-subsection \<open>Unsigned Bitwise Operations\<close>
+subsection \<open>Unsigned bitwise operations\<close>
 
 lemma wp_c_unsigned_and [micro_rust_wp_simps]:
-  fixes a b :: \<open>'l::{len} word\<close>
+    fixes a b :: \<open>'l::{len} word\<close>
   assumes \<open>\<And>r. ucincl (\<psi> r)\<close>
-  shows \<open>\<W>\<P> \<Gamma> (c_unsigned_and a b) \<psi> \<rho> \<theta> = \<psi> (a AND b)\<close>
-  using assms by (simp add: c_unsigned_and_def micro_rust_wp_simps)
+    shows \<open>\<W>\<P> \<Gamma> (c_unsigned_and a b) \<psi> \<rho> \<theta> = \<psi> (a AND b)\<close>
+using assms by (simp add: c_unsigned_and_def micro_rust_wp_simps asepconj_simp)
 
 lemma wp_c_unsigned_andI [micro_rust_wp_intros]:
-  fixes a b :: \<open>'l::{len} word\<close>
-  assumes \<open>\<phi> \<longlongrightarrow> \<psi> (a AND b) \<star> \<top>\<close>
-  shows \<open>\<phi> \<longlongrightarrow> \<W>\<P> \<Gamma> (c_unsigned_and a b) \<psi> \<rho> \<theta>\<close>
-  using assms by (simp add: c_unsigned_and_def wp_literalI)
+    fixes a b :: \<open>'l::{len} word\<close>
+  assumes \<open>\<And>r. ucincl (\<psi> r)\<close>
+      and \<open>\<phi> \<longlongrightarrow> \<psi> (a AND b)\<close>
+    shows \<open>\<phi> \<longlongrightarrow> \<W>\<P> \<Gamma> (c_unsigned_and a b) \<psi> \<rho> \<theta>\<close>
+using assms by (simp add: c_unsigned_and_def wp_literalI asepconj_simp)
 
 lemma wp_c_unsigned_or [micro_rust_wp_simps]:
-  fixes a b :: \<open>'l::{len} word\<close>
+    fixes a b :: \<open>'l::{len} word\<close>
   assumes \<open>\<And>r. ucincl (\<psi> r)\<close>
-  shows \<open>\<W>\<P> \<Gamma> (c_unsigned_or a b) \<psi> \<rho> \<theta> = \<psi> (a OR b)\<close>
-  using assms by (simp add: c_unsigned_or_def micro_rust_wp_simps)
+    shows \<open>\<W>\<P> \<Gamma> (c_unsigned_or a b) \<psi> \<rho> \<theta> = \<psi> (a OR b)\<close>
+using assms by (simp add: c_unsigned_or_def micro_rust_wp_simps)
 
 lemma wp_c_unsigned_orI [micro_rust_wp_intros]:
-  fixes a b :: \<open>'l::{len} word\<close>
-  assumes \<open>\<phi> \<longlongrightarrow> \<psi> (a OR b) \<star> \<top>\<close>
-  shows \<open>\<phi> \<longlongrightarrow> \<W>\<P> \<Gamma> (c_unsigned_or a b) \<psi> \<rho> \<theta>\<close>
-  using assms by (simp add: c_unsigned_or_def wp_literalI)
+    fixes a b :: \<open>'l::{len} word\<close>
+  assumes \<open>\<And>r. ucincl (\<psi> r)\<close>
+      and \<open>\<phi> \<longlongrightarrow> \<psi> (a OR b)\<close>
+    shows \<open>\<phi> \<longlongrightarrow> \<W>\<P> \<Gamma> (c_unsigned_or a b) \<psi> \<rho> \<theta>\<close>
+using assms by (simp add: c_unsigned_or_def wp_literalI asepconj_simp)
 
 lemma wp_c_unsigned_xor [micro_rust_wp_simps]:
-  fixes a b :: \<open>'l::{len} word\<close>
+    fixes a b :: \<open>'l::{len} word\<close>
   assumes \<open>\<And>r. ucincl (\<psi> r)\<close>
-  shows \<open>\<W>\<P> \<Gamma> (c_unsigned_xor a b) \<psi> \<rho> \<theta> = \<psi> (a XOR b)\<close>
-  using assms by (simp add: c_unsigned_xor_def micro_rust_wp_simps)
+    shows \<open>\<W>\<P> \<Gamma> (c_unsigned_xor a b) \<psi> \<rho> \<theta> = \<psi> (a XOR b)\<close>
+using assms by (simp add: c_unsigned_xor_def micro_rust_wp_simps)
 
 lemma wp_c_unsigned_xorI [micro_rust_wp_intros]:
-  fixes a b :: \<open>'l::{len} word\<close>
-  assumes \<open>\<phi> \<longlongrightarrow> \<psi> (a XOR b) \<star> \<top>\<close>
-  shows \<open>\<phi> \<longlongrightarrow> \<W>\<P> \<Gamma> (c_unsigned_xor a b) \<psi> \<rho> \<theta>\<close>
-  using assms by (simp add: c_unsigned_xor_def wp_literalI)
+    fixes a b :: \<open>'l::{len} word\<close>
+  assumes \<open>\<And>r. ucincl (\<psi> r)\<close>
+      and \<open>\<phi> \<longlongrightarrow> \<psi> (a XOR b)\<close>
+    shows \<open>\<phi> \<longlongrightarrow> \<W>\<P> \<Gamma> (c_unsigned_xor a b) \<psi> \<rho> \<theta>\<close>
+using assms by (simp add: c_unsigned_xor_def wp_literalI asepconj_simp)
 
 lemma wp_c_unsigned_not [micro_rust_wp_simps]:
-  fixes a :: \<open>'l::{len} word\<close>
+    fixes a :: \<open>'l::{len} word\<close>
   assumes \<open>\<And>r. ucincl (\<psi> r)\<close>
-  shows \<open>\<W>\<P> \<Gamma> (c_unsigned_not a) \<psi> \<rho> \<theta> = \<psi> (NOT a)\<close>
-  using assms by (simp add: c_unsigned_not_def micro_rust_wp_simps)
+    shows \<open>\<W>\<P> \<Gamma> (c_unsigned_not a) \<psi> \<rho> \<theta> = \<psi> (NOT a)\<close>
+using assms by (simp add: c_unsigned_not_def micro_rust_wp_simps)
 
 lemma wp_c_unsigned_notI [micro_rust_wp_intros]:
-  fixes a :: \<open>'l::{len} word\<close>
-  assumes \<open>\<phi> \<longlongrightarrow> \<psi> (NOT a) \<star> \<top>\<close>
-  shows \<open>\<phi> \<longlongrightarrow> \<W>\<P> \<Gamma> (c_unsigned_not a) \<psi> \<rho> \<theta>\<close>
-  using assms by (simp add: c_unsigned_not_def wp_literalI)
+    fixes a :: \<open>'l::{len} word\<close>
+  assumes \<open>\<And>r. ucincl (\<psi> r)\<close>
+      and \<open>\<phi> \<longlongrightarrow> \<psi> (NOT a)\<close>
+    shows \<open>\<phi> \<longlongrightarrow> \<W>\<P> \<Gamma> (c_unsigned_not a) \<psi> \<rho> \<theta>\<close>
+using assms by (simp add: c_unsigned_not_def wp_literalI asepconj_simp)
 
 subsection \<open>Unsigned Shift Operations\<close>
 
 lemma wp_c_unsigned_shl [micro_rust_wp_simps]:
-  fixes a b :: \<open>'l::{len} word\<close>
+    fixes a b :: \<open>'l::{len} word\<close>
   assumes \<open>\<And>r. ucincl (\<psi> r)\<close>
-  shows \<open>\<W>\<P> \<Gamma> (c_unsigned_shl a b) \<psi> \<rho> \<theta> =
-    (if unat b < LENGTH('l)
-     then \<psi> (push_bit (unat b) a)
-     else \<theta> (CustomAbort ShiftOutOfRange) \<star> UNIV)\<close>
-  using assms
-  by (simp add: c_unsigned_shl_def c_shift_out_of_range_def c_abort_def micro_rust_wp_simps)
+      and \<open>\<And>r. ucincl (\<theta> r)\<close>
+    shows \<open>\<W>\<P> \<Gamma> (c_unsigned_shl a b) \<psi> \<rho> \<theta> = 
+            (if unat b < LENGTH('l) then
+               \<psi> (push_bit (unat b) a)
+             else
+               \<theta> (CustomAbort ShiftOutOfRange))\<close>
+using assms by (simp add: c_unsigned_shl_def c_shift_out_of_range_def c_abort_def micro_rust_wp_simps
+  asepconj_simp)
 
 lemma wp_c_unsigned_shlI [micro_rust_wp_intros]:
-  fixes a b :: \<open>'l::{len} word\<close>
-  assumes \<open>unat b < LENGTH('l)\<close>
-      and \<open>\<phi> \<longlongrightarrow> \<psi> (push_bit (unat b) a) \<star> \<top>\<close>
-  shows \<open>\<phi> \<longlongrightarrow> \<W>\<P> \<Gamma> (c_unsigned_shl a b) \<psi> \<rho> \<theta>\<close>
+    fixes a b :: \<open>'l::{len} word\<close>
+  assumes \<open>\<And>r. ucincl (\<psi> r)\<close>
+      and \<open>unat b < LENGTH('l)\<close>
+      and \<open>\<phi> \<longlongrightarrow> \<psi> (push_bit (unat b) a)\<close>
+    shows \<open>\<phi> \<longlongrightarrow> \<W>\<P> \<Gamma> (c_unsigned_shl a b) \<psi> \<rho> \<theta>\<close>
 proof -
-  from assms(1) have eq: \<open>c_unsigned_shl a b = literal (push_bit (unat b) a)\<close>
+  from assms have eq: \<open>c_unsigned_shl a b = literal (push_bit (unat b) a)\<close>
     by (simp add: c_unsigned_shl_def)
-  show ?thesis unfolding eq using assms(2) by (rule wp_literalI)
+  from this assms show ?thesis
+    unfolding eq using assms by (auto intro: wp_literalI simp add: asepconj_simp)
 qed
 
 lemma wp_c_unsigned_shr [micro_rust_wp_simps]:
-  fixes a b :: \<open>'l::{len} word\<close>
+    fixes a b :: \<open>'l::{len} word\<close>
   assumes \<open>\<And>r. ucincl (\<psi> r)\<close>
-  shows \<open>\<W>\<P> \<Gamma> (c_unsigned_shr a b) \<psi> \<rho> \<theta> =
-    (if unat b < LENGTH('l)
-     then \<psi> (drop_bit (unat b) a)
-     else \<theta> (CustomAbort ShiftOutOfRange) \<star> UNIV)\<close>
-  using assms
-  by (simp add: c_unsigned_shr_def c_shift_out_of_range_def c_abort_def micro_rust_wp_simps)
+      and \<open>\<And>r. ucincl (\<theta> r)\<close>
+    shows \<open>\<W>\<P> \<Gamma> (c_unsigned_shr a b) \<psi> \<rho> \<theta> =
+             (if unat b < LENGTH('l) then
+                \<psi> (drop_bit (unat b) a)
+              else \<theta> (CustomAbort ShiftOutOfRange))\<close>
+using assms by (simp add: c_unsigned_shr_def c_shift_out_of_range_def c_abort_def
+  micro_rust_wp_simps asepconj_simp)
 
 lemma wp_c_unsigned_shrI [micro_rust_wp_intros]:
   fixes a b :: \<open>'l::{len} word\<close>
-  assumes \<open>unat b < LENGTH('l)\<close>
-      and \<open>\<phi> \<longlongrightarrow> \<psi> (drop_bit (unat b) a) \<star> \<top>\<close>
-  shows \<open>\<phi> \<longlongrightarrow> \<W>\<P> \<Gamma> (c_unsigned_shr a b) \<psi> \<rho> \<theta>\<close>
+  assumes \<open>\<And>r. ucincl (\<psi> r)\<close>
+      and \<open>unat b < LENGTH('l)\<close>
+      and \<open>\<phi> \<longlongrightarrow> \<psi> (drop_bit (unat b) a)\<close>
+    shows \<open>\<phi> \<longlongrightarrow> \<W>\<P> \<Gamma> (c_unsigned_shr a b) \<psi> \<rho> \<theta>\<close>
 proof -
-  from assms(1) have eq: \<open>c_unsigned_shr a b = literal (drop_bit (unat b) a)\<close>
+  from assms have eq: \<open>c_unsigned_shr a b = literal (drop_bit (unat b) a)\<close>
     by (simp add: c_unsigned_shr_def)
-  show ?thesis unfolding eq using assms(2) by (rule wp_literalI)
+  from this assms show ?thesis
+    unfolding eq by (auto intro: wp_literalI simp add: asepconj_simp)
 qed
 
-subsection \<open>Signed Shift Operations\<close>
+subsection \<open>Signed shift operations\<close>
 
 lemma wp_c_signed_shl [micro_rust_wp_simps]:
-  fixes a b :: \<open>'l::{len} sword\<close>
+    fixes a b :: \<open>'l::{len} sword\<close>
   assumes \<open>\<And>r. ucincl (\<psi> r)\<close>
-  shows \<open>\<W>\<P> \<Gamma> (c_signed_shl a b) \<psi> \<rho> \<theta> =
-    (if unat b \<ge> LENGTH('l) then \<theta> (CustomAbort ShiftOutOfRange) \<star> UNIV
-     else let result_int = sint a * 2 ^ unat b in
-       if sint a < 0 \<or> \<not> c_signed_in_range result_int LENGTH('l) then
-         \<theta> (CustomAbort SignedOverflow) \<star> UNIV
-       else \<psi> (word_of_int result_int))\<close>
-  using assms
-  by (simp add: c_signed_shl_def c_shift_out_of_range_def c_signed_overflow_def
-                c_abort_def Let_def micro_rust_wp_simps)
+      and \<open>\<And>r. ucincl (\<theta> r)\<close>
+    shows \<open>\<W>\<P> \<Gamma> (c_signed_shl a b) \<psi> \<rho> \<theta> =
+            (if unat b \<ge> LENGTH('l) then
+               \<theta> (CustomAbort ShiftOutOfRange)
+             else
+               let result_int = sint a * 2 ^ unat b in
+                 if sint a < 0 \<or> \<not> c_signed_in_range result_int LENGTH('l) then
+                   \<theta> (CustomAbort SignedOverflow)
+                 else
+                   \<psi> (word_of_int result_int))\<close>
+using assms by (simp add: c_signed_shl_def c_shift_out_of_range_def c_signed_overflow_def
+                c_abort_def Let_def micro_rust_wp_simps asepconj_simp)
 
 lemma wp_c_signed_shlI [micro_rust_wp_intros]:
-  fixes a b :: \<open>'l::{len} sword\<close>
-  assumes \<open>unat b < LENGTH('l)\<close>
+    fixes a b :: \<open>'l::{len} sword\<close>
+  assumes \<open>\<And>r. ucincl (\<psi> r)\<close>
+      and \<open>unat b < LENGTH('l)\<close>
       and \<open>sint a \<ge> 0\<close>
       and \<open>c_signed_in_range (sint a * 2 ^ unat b) LENGTH('l)\<close>
-      and \<open>\<phi> \<longlongrightarrow> \<psi> (word_of_int (sint a * 2 ^ unat b)) \<star> \<top>\<close>
-  shows \<open>\<phi> \<longlongrightarrow> \<W>\<P> \<Gamma> (c_signed_shl a b) \<psi> \<rho> \<theta>\<close>
+      and \<open>\<phi> \<longlongrightarrow> \<psi> (word_of_int (sint a * 2 ^ unat b))\<close>
+    shows \<open>\<phi> \<longlongrightarrow> \<W>\<P> \<Gamma> (c_signed_shl a b) \<psi> \<rho> \<theta>\<close>
 proof -
-  from assms(1,2,3) have eq: \<open>c_signed_shl a b = literal (word_of_int (sint a * 2 ^ unat b))\<close>
+  from assms have eq: \<open>c_signed_shl a b = literal (word_of_int (sint a * 2 ^ unat b))\<close>
     by (simp add: c_signed_shl_def c_shift_out_of_range_def c_signed_overflow_def Let_def)
-  show ?thesis unfolding eq using assms(4) by (rule wp_literalI)
+  from this assms show ?thesis
+    unfolding eq by (auto intro: wp_literalI simp add: asepconj_simp)
 qed
 
 lemma wp_c_signed_shr [micro_rust_wp_simps]:
-  fixes a b :: \<open>'l::{len} sword\<close>
+    fixes a b :: \<open>'l::{len} sword\<close>
   assumes \<open>\<And>r. ucincl (\<psi> r)\<close>
-  shows \<open>\<W>\<P> \<Gamma> (c_signed_shr a b) \<psi> \<rho> \<theta> =
-    (if unat b \<ge> LENGTH('l) then \<theta> (CustomAbort ShiftOutOfRange) \<star> UNIV
-     else \<psi> (word_of_int (sint a div 2 ^ unat b)))\<close>
-  using assms
-  by (simp add: c_signed_shr_def c_shift_out_of_range_def
-                c_abort_def micro_rust_wp_simps)
+      and \<open>\<And>r. ucincl (\<theta> r)\<close>
+    shows \<open>\<W>\<P> \<Gamma> (c_signed_shr a b) \<psi> \<rho> \<theta> =
+             (if unat b \<ge> LENGTH('l) then
+                \<theta> (CustomAbort ShiftOutOfRange)
+              else
+                \<psi> (word_of_int (sint a div 2 ^ unat b)))\<close>
+using assms by (simp add: c_signed_shr_def c_shift_out_of_range_def c_abort_def micro_rust_wp_simps
+  asepconj_simp)
 
 lemma wp_c_signed_shrI [micro_rust_wp_intros]:
-  fixes a b :: \<open>'l::{len} sword\<close>
-  assumes \<open>unat b < LENGTH('l)\<close>
-      and \<open>\<phi> \<longlongrightarrow> \<psi> (word_of_int (sint a div 2 ^ unat b)) \<star> \<top>\<close>
-  shows \<open>\<phi> \<longlongrightarrow> \<W>\<P> \<Gamma> (c_signed_shr a b) \<psi> \<rho> \<theta>\<close>
+    fixes a b :: \<open>'l::{len} sword\<close>
+  assumes \<open>\<And>r. ucincl (\<psi> r)\<close>
+      and \<open>unat b < LENGTH('l)\<close>
+      and \<open>\<phi> \<longlongrightarrow> \<psi> (word_of_int (sint a div 2 ^ unat b))\<close>
+    shows \<open>\<phi> \<longlongrightarrow> \<W>\<P> \<Gamma> (c_signed_shr a b) \<psi> \<rho> \<theta>\<close>
 proof -
-  from assms(1) have eq: \<open>c_signed_shr a b = literal (word_of_int (sint a div 2 ^ unat b))\<close>
+  from assms have eq: \<open>c_signed_shr a b = literal (word_of_int (sint a div 2 ^ unat b))\<close>
     by (simp add: c_signed_shr_def c_shift_out_of_range_def)
-  show ?thesis unfolding eq using assms(2) by (rule wp_literalI)
+  from assms this show ?thesis
+    unfolding eq by (auto intro: wp_literalI simp add: asepconj_simp)
 qed
 
-subsection \<open>Type Cast Operations\<close>
+subsection \<open>Type cast operations\<close>
 
 lemma wp_c_ucast [micro_rust_wp_simps]:
   assumes \<open>\<And>r. ucincl (\<psi> r)\<close>
-  shows \<open>\<W>\<P> \<Gamma> (c_ucast w) \<psi> \<rho> \<theta> = \<psi> (ucast w)\<close>
-  using assms by (simp add: c_ucast_def micro_rust_wp_simps)
+    shows \<open>\<W>\<P> \<Gamma> (c_ucast w) \<psi> \<rho> \<theta> = \<psi> (ucast w)\<close>
+using assms by (simp add: c_ucast_def micro_rust_wp_simps)
 
 lemma wp_c_ucastI [micro_rust_wp_intros]:
-  assumes \<open>\<phi> \<longlongrightarrow> \<psi> (ucast w) \<star> \<top>\<close>
-  shows \<open>\<phi> \<longlongrightarrow> \<W>\<P> \<Gamma> (c_ucast w) \<psi> \<rho> \<theta>\<close>
-  using assms by (simp add: c_ucast_def wp_literalI)
+  assumes \<open>\<And>r. ucincl (\<psi> r)\<close>
+      and \<open>\<phi> \<longlongrightarrow> \<psi> (ucast w)\<close>
+    shows \<open>\<phi> \<longlongrightarrow> \<W>\<P> \<Gamma> (c_ucast w) \<psi> \<rho> \<theta>\<close>
+using assms by (simp add: c_ucast_def wp_literalI asepconj_simp)
 
 lemma wp_c_scast [micro_rust_wp_simps]:
   assumes \<open>\<And>r. ucincl (\<psi> r)\<close>
-  shows \<open>\<W>\<P> \<Gamma> (c_scast w) \<psi> \<rho> \<theta> = \<psi> (scast w)\<close>
-  using assms by (simp add: c_scast_def micro_rust_wp_simps)
+    shows \<open>\<W>\<P> \<Gamma> (c_scast w) \<psi> \<rho> \<theta> = \<psi> (scast w)\<close>
+using assms by (simp add: c_scast_def micro_rust_wp_simps)
 
 lemma wp_c_scastI [micro_rust_wp_intros]:
-  assumes \<open>\<phi> \<longlongrightarrow> \<psi> (scast w) \<star> \<top>\<close>
-  shows \<open>\<phi> \<longlongrightarrow> \<W>\<P> \<Gamma> (c_scast w) \<psi> \<rho> \<theta>\<close>
-  using assms by (simp add: c_scast_def wp_literalI)
+  assumes \<open>\<And>r. ucincl (\<psi> r)\<close>
+      and \<open>\<phi> \<longlongrightarrow> \<psi> (scast w)\<close>
+    shows \<open>\<phi> \<longlongrightarrow> \<W>\<P> \<Gamma> (c_scast w) \<psi> \<rho> \<theta>\<close>
+using assms by (simp add: c_scast_def wp_literalI asepconj_simp)
 
 subsection \<open>Unsigned Division and Modulo\<close>
 
 lemma wp_c_unsigned_div [micro_rust_wp_simps]:
-  fixes a b :: \<open>'l::{len} word\<close>
+    fixes a b :: \<open>'l::{len} word\<close>
   assumes \<open>\<And>r. ucincl (\<psi> r)\<close>
-  shows \<open>\<W>\<P> \<Gamma> (c_unsigned_div a b) \<psi> \<rho> \<theta> =
-    (if b = 0 then \<theta> (CustomAbort DivisionByZero) \<star> UNIV
-     else \<psi> (a div b))\<close>
-  using assms
-  by (simp add: c_unsigned_div_def c_abort_def c_division_by_zero_def micro_rust_wp_simps)
+      and \<open>\<And>r. ucincl (\<theta> r)\<close>
+    shows \<open>\<W>\<P> \<Gamma> (c_unsigned_div a b) \<psi> \<rho> \<theta> =
+             (if b = 0 then
+                \<theta> (CustomAbort DivisionByZero)
+              else
+                \<psi> (a div b))\<close>
+using assms by (simp add: c_unsigned_div_def c_abort_def c_division_by_zero_def micro_rust_wp_simps
+  asepconj_simp)
 
 lemma wp_c_unsigned_mod [micro_rust_wp_simps]:
-  fixes a b :: \<open>'l::{len} word\<close>
+    fixes a b :: \<open>'l::{len} word\<close>
   assumes \<open>\<And>r. ucincl (\<psi> r)\<close>
-  shows \<open>\<W>\<P> \<Gamma> (c_unsigned_mod a b) \<psi> \<rho> \<theta> =
-    (if b = 0 then \<theta> (CustomAbort DivisionByZero) \<star> UNIV
-     else \<psi> (a mod b))\<close>
-  using assms
-  by (simp add: c_unsigned_mod_def c_abort_def c_division_by_zero_def micro_rust_wp_simps)
+      and \<open>\<And>r. ucincl (\<theta> r)\<close>
+    shows \<open>\<W>\<P> \<Gamma> (c_unsigned_mod a b) \<psi> \<rho> \<theta> =
+             (if b = 0 then
+                \<theta> (CustomAbort DivisionByZero)
+              else
+                \<psi> (a mod b))\<close>
+using assms by (simp add: c_unsigned_mod_def c_abort_def c_division_by_zero_def micro_rust_wp_simps
+  asepconj_simp)
 
 section \<open>C Integer Promotion Lemmas\<close>
 
@@ -552,24 +597,19 @@ subsection \<open>Signed 16 to 32 promotion roundtrip\<close>
 
 lemma scast_scast_add_roundtrip_16_32 [simp]:
   fixes a b :: \<open>16 sword\<close>
-  shows \<open>SCAST(32 signed \<rightarrow> 16 signed)
-         (SCAST(16 signed \<rightarrow> 32 signed) a + SCAST(16 signed \<rightarrow> 32 signed) b)
-       = a + b\<close>
-  by (simp add: scast_down_add scast_up_scast_id is_up is_down)
+  shows \<open>SCAST(32 signed \<rightarrow> 16 signed) (SCAST(16 signed \<rightarrow> 32 signed) a + SCAST(16 signed \<rightarrow> 32 signed) b) = a + b\<close>
+by (simp add: scast_down_add scast_up_scast_id is_up is_down)
 
 lemma scast_scast_sub_roundtrip_16_32 [simp]:
   fixes a b :: \<open>16 sword\<close>
-  shows \<open>SCAST(32 signed \<rightarrow> 16 signed)
-         (SCAST(16 signed \<rightarrow> 32 signed) a - SCAST(16 signed \<rightarrow> 32 signed) b)
-       = a - b\<close>
-  by (simp add: scast_down_minus scast_up_scast_id is_up is_down)
+  shows \<open>SCAST(32 signed \<rightarrow> 16 signed) (SCAST(16 signed \<rightarrow> 32 signed) a - SCAST(16 signed \<rightarrow> 32 signed) b) = a - b\<close>
+by (simp add: scast_down_minus scast_up_scast_id is_up is_down)
 
 subsection \<open>32-bit signed overflow bounds for promoted 16-bit signed values\<close>
 
 lemma sint_scast_16_32_add_upper [simp]:
   fixes a b :: \<open>16 sword\<close>
-  shows \<open>sint (SCAST(16 signed \<rightarrow> 32 signed) a)
-       + sint (SCAST(16 signed \<rightarrow> 32 signed) b) < 2147483648\<close>
+  shows \<open>sint (SCAST(16 signed \<rightarrow> 32 signed) a) + sint (SCAST(16 signed \<rightarrow> 32 signed) b) < 2147483648\<close>
 proof -
   have \<open>sint (SCAST(16 signed \<rightarrow> 32 signed) a) = sint a\<close>
     by (simp add: sint_up_scast is_up)
@@ -579,14 +619,13 @@ proof -
     using sint_range_size[where w=a] by (simp add: word_size)
   moreover have \<open>sint b \<ge> -32768 \<and> sint b \<le> 32767\<close>
     using sint_range_size[where w=b] by (simp add: word_size)
-  ultimately show ?thesis by linarith
+  ultimately show ?thesis
+    by linarith
 qed
 
 lemma sint_scast_16_32_add_lower [simp]:
   fixes a b :: \<open>16 sword\<close>
-  shows \<open>- 2147483648
-       \<le> sint (SCAST(16 signed \<rightarrow> 32 signed) a)
-        + sint (SCAST(16 signed \<rightarrow> 32 signed) b)\<close>
+  shows \<open>- 2147483648 \<le> sint (SCAST(16 signed \<rightarrow> 32 signed) a) + sint (SCAST(16 signed \<rightarrow> 32 signed) b)\<close>
 proof -
   have \<open>sint (SCAST(16 signed \<rightarrow> 32 signed) a) = sint a\<close>
     by (simp add: sint_up_scast is_up)
@@ -596,13 +635,13 @@ proof -
     using sint_range_size[where w=a] by (simp add: word_size)
   moreover have \<open>sint b \<ge> -32768\<close>
     using sint_range_size[where w=b] by (simp add: word_size)
-  ultimately show ?thesis by linarith
+  ultimately show ?thesis
+    by linarith
 qed
 
 lemma sint_scast_16_32_sub_upper [simp]:
   fixes a b :: \<open>16 sword\<close>
-  shows \<open>sint (SCAST(16 signed \<rightarrow> 32 signed) a)
-       - sint (SCAST(16 signed \<rightarrow> 32 signed) b) < 2147483648\<close>
+  shows \<open>sint (SCAST(16 signed \<rightarrow> 32 signed) a) - sint (SCAST(16 signed \<rightarrow> 32 signed) b) < 2147483648\<close>
 proof -
   have \<open>sint (SCAST(16 signed \<rightarrow> 32 signed) a) = sint a\<close>
     by (simp add: sint_up_scast is_up)
@@ -612,14 +651,13 @@ proof -
     using sint_range_size[where w=a] by (simp add: word_size)
   moreover have \<open>sint b \<ge> -32768\<close>
     using sint_range_size[where w=b] by (simp add: word_size)
-  ultimately show ?thesis by linarith
+  ultimately show ?thesis
+    by linarith
 qed
 
 lemma sint_scast_16_32_sub_lower [simp]:
   fixes a b :: \<open>16 sword\<close>
-  shows \<open>- 2147483648
-       \<le> sint (SCAST(16 signed \<rightarrow> 32 signed) a)
-        - sint (SCAST(16 signed \<rightarrow> 32 signed) b)\<close>
+  shows \<open>- 2147483648 \<le> sint (SCAST(16 signed \<rightarrow> 32 signed) a) - sint (SCAST(16 signed \<rightarrow> 32 signed) b)\<close>
 proof -
   have \<open>sint (SCAST(16 signed \<rightarrow> 32 signed) a) = sint a\<close>
     by (simp add: sint_up_scast is_up)
@@ -629,7 +667,8 @@ proof -
     using sint_range_size[where w=a] by (simp add: word_size)
   moreover have \<open>sint b \<le> 32767\<close>
     using sint_range_size[where w=b] by (simp add: word_size)
-  ultimately show ?thesis by linarith
+  ultimately show ?thesis
+    by linarith
 qed
 
 subsection \<open>Unsigned 16 to signed 32 promotion roundtrip\<close>
@@ -637,19 +676,16 @@ subsection \<open>Unsigned 16 to signed 32 promotion roundtrip\<close>
 lemma scast_ucast_roundtrip_16_32:
   fixes a :: \<open>16 word\<close>
   shows \<open>SCAST(32 signed \<rightarrow> 16) (UCAST(16 \<rightarrow> 32 signed) a) = a\<close>
-  by (simp add: scast_def sint_ucast_eq_uint is_down word_of_int_uint)
+by (simp add: scast_def sint_ucast_eq_uint is_down word_of_int_uint)
 
 lemma scast_ucast_add_roundtrip_16_32 [simp]:
   fixes a b :: \<open>16 word\<close>
-  shows \<open>SCAST(32 signed \<rightarrow> 16)
-         (UCAST(16 \<rightarrow> 32 signed) a + UCAST(16 \<rightarrow> 32 signed) b)
-       = a + b\<close>
-  by (simp add: scast_down_add is_down scast_ucast_roundtrip_16_32)
+  shows \<open>SCAST(32 signed \<rightarrow> 16) (UCAST(16 \<rightarrow> 32 signed) a + UCAST(16 \<rightarrow> 32 signed) b) = a + b\<close>
+by (simp add: scast_down_add is_down scast_ucast_roundtrip_16_32)
 
 lemma sint_ucast_16_32_add_upper [simp]:
   fixes a b :: \<open>16 word\<close>
-  shows \<open>sint (UCAST(16 \<rightarrow> 32 signed) a)
-       + sint (UCAST(16 \<rightarrow> 32 signed) b) < 2147483648\<close>
+  shows \<open>sint (UCAST(16 \<rightarrow> 32 signed) a) + sint (UCAST(16 \<rightarrow> 32 signed) b) < 2147483648\<close>
 proof -
   have \<open>sint (UCAST(16 \<rightarrow> 32 signed) a) = uint a\<close>
     by (simp add: sint_ucast_eq_uint is_down)
@@ -659,22 +695,24 @@ proof -
     using uint_range_size[where w=a] by (simp add: word_size)
   moreover have \<open>uint b < 65536\<close>
     using uint_range_size[where w=b] by (simp add: word_size)
-  ultimately show ?thesis by linarith
+  ultimately show ?thesis
+    by linarith
 qed
 
 lemma sint_ucast_16_32_add_lower [simp]:
   fixes a b :: \<open>16 word\<close>
-  shows \<open>- 2147483648
-       \<le> sint (UCAST(16 \<rightarrow> 32 signed) a)
-        + sint (UCAST(16 \<rightarrow> 32 signed) b)\<close>
+  shows \<open>- 2147483648 \<le> sint (UCAST(16 \<rightarrow> 32 signed) a) + sint (UCAST(16 \<rightarrow> 32 signed) b)\<close>
 proof -
   have \<open>sint (UCAST(16 \<rightarrow> 32 signed) a) = uint a\<close>
     by (simp add: sint_ucast_eq_uint is_down)
   moreover have \<open>sint (UCAST(16 \<rightarrow> 32 signed) b) = uint b\<close>
     by (simp add: sint_ucast_eq_uint is_down)
-  moreover have \<open>uint a \<ge> 0\<close> by simp
-  moreover have \<open>uint b \<ge> 0\<close> by simp
-  ultimately show ?thesis by linarith
+  moreover have \<open>uint a \<ge> 0\<close>
+    by simp
+  moreover have \<open>uint b \<ge> 0\<close>
+    by simp
+  ultimately show ?thesis
+    by linarith
 qed
 
 end
