Shallow_Micro_C/C_Pointer_Types.thy
@@ -1,6 +1,3 @@
-(* Copyright Amazon.com, Inc. or its affiliates. All Rights Reserved.
-   SPDX-License-Identifier: MIT *)
-
 theory C_Pointer_Types
   imports
     C_Abort
@@ -15,7 +12,7 @@ text \<open>
   with @{const NullPointerDereference} on null pointer access.
 \<close>
 
-subsection \<open>Null Pointer\<close>
+subsection \<open>Null pointer\<close>
 
 text \<open>
   We define null as the zero address for numeric address types.
@@ -27,10 +24,11 @@ definition c_null :: \<open>(nat, 'b) gref\<close> where
 definition is_null_nat :: \<open>(nat, 'b) gref \<Rightarrow> bool\<close> where
   \<open>is_null_nat p \<equiv> address p = 0\<close>
 
-lemma is_null_c_null [simp]: \<open>is_null_nat c_null\<close>
-  by (simp add: is_null_nat_def c_null_def gref.sel)
+lemma is_null_c_null [simp]:
+  shows \<open>is_null_nat c_null\<close>
+by (simp add: is_null_nat_def c_null_def gref.sel)
 
-subsection \<open>Null-Checked Pointer Operations\<close>
+subsection \<open>Null-checked pointer operations\<close>
 
 text \<open>
   These operations check for null before performing the underlying memory
@@ -39,11 +37,13 @@ text \<open>
   can be composed with any locale-provided dereference or update.
 \<close>
 
-definition c_null_guard :: \<open>(nat, 'b) gref \<Rightarrow>
-    ((nat, 'b) gref \<Rightarrow> ('s, 'v, 'r, c_abort, 'i, 'o) expression) \<Rightarrow>
+definition c_null_guard :: \<open>(nat, 'b) gref \<Rightarrow> ((nat, 'b) gref \<Rightarrow>
+    ('s, 'v, 'r, c_abort, 'i, 'o) expression) \<Rightarrow>
     ('s, 'v, 'r, c_abort, 'i, 'o) expression\<close> where
   \<open>c_null_guard p op \<equiv>
-     if is_null_nat p then c_null_pointer_dereference
-     else op p\<close>
+     if is_null_nat p then
+       c_null_pointer_dereference
+     else
+      op p\<close>
 
 end
