Shallow_Micro_C/Shallow_Micro_C.thy
@@ -1,6 +1,3 @@
-(* Copyright Amazon.com, Inc. or its affiliates. All Rights Reserved.
-   SPDX-License-Identifier: MIT *)
-
 theory Shallow_Micro_C
   imports
     C_Abort
